no draws

.lake/build/ir/Games/gameLib/Conditioning.c
@@ -13,86 +13,119 @@
 #ifdef __cplusplus
 extern "C" {
 #endif
-LEAN_EXPORT lean_object* l_zGame__World__wDraw_world__after__fst___rarg(lean_object*, lean_object*, lean_object*);
+LEAN_EXPORT lean_object* l_Game__World_world__after__fst___elambda__2___rarg(lean_object*, lean_object*, lean_object*, lean_object*);
+LEAN_EXPORT lean_object* l_Game__World_world__after__preHist___elambda__2(lean_object*, lean_object*);
 lean_object* lean_mk_empty_array_with_capacity(lean_object*);
 LEAN_EXPORT lean_object* l_fst__strat__deconditioned(lean_object*, lean_object*);
-LEAN_EXPORT lean_object* l_zGame__World__wDraw_snd__strat__conditioned___rarg(lean_object*, lean_object*, lean_object*, lean_object*, lean_object*);
-LEAN_EXPORT lean_object* l_zGame__wDraw_state__on__turn___rarg(lean_object*, lean_object*);
-LEAN_EXPORT lean_object* l_zGame__wDraw_history__on__turn___rarg___boxed(lean_object*, lean_object*);
-LEAN_EXPORT lean_object* l_zGame__World__wDraw_snd__strat__conditioned___rarg___boxed(lean_object*, lean_object*, lean_object*, lean_object*, lean_object*);
 LEAN_EXPORT lean_object* l___private_Games_gameLib_Conditioning_0__History__on__turn_match__1_splitter(lean_object*);
+LEAN_EXPORT lean_object* l_zGame_state__on__turn___rarg(lean_object*, lean_object*);
+LEAN_EXPORT lean_object* l_zGame_history__on__turn(lean_object*, lean_object*);
 LEAN_EXPORT uint8_t l_instDecidableEqListNil___rarg(lean_object*);
-LEAN_EXPORT lean_object* l_Game__World__wDraw_world__after__fst(lean_object*, lean_object*);
 LEAN_EXPORT lean_object* l___private_Games_gameLib_Conditioning_0__History__on__turn_match__1_splitter___rarg___boxed(lean_object*, lean_object*, lean_object*);
-LEAN_EXPORT lean_object* l_zGame__World__wDraw_snd__strat__conditioned(lean_object*, lean_object*);
+LEAN_EXPORT lean_object* l_Game__World_world__after__preHist___elambda__1___rarg(lean_object*, lean_object*, lean_object*, lean_object*);
+LEAN_EXPORT lean_object* l_Game__World_world__after__preHist___rarg(lean_object*, lean_object*);
 lean_object* l_List_appendTR___rarg(lean_object*, lean_object*);
 uint8_t l_instDecidablePredNatTurn__fst(lean_object*);
+LEAN_EXPORT lean_object* l_zGame__World_snd__strat__deconditioned(lean_object*, lean_object*);
 LEAN_EXPORT lean_object* l_instDecidableEqListNil___rarg___boxed(lean_object*);
+LEAN_EXPORT lean_object* l_Game__World_world__after__fst___rarg(lean_object*, lean_object*);
+LEAN_EXPORT lean_object* l_Game__World_world__after__preHist___elambda__1(lean_object*, lean_object*);
 lean_object* lean_array_pop(lean_object*);
+LEAN_EXPORT lean_object* l_zGame__World_world__after__fst___rarg(lean_object*, lean_object*, lean_object*);
 lean_object* lean_array_to_list(lean_object*, lean_object*);
-LEAN_EXPORT lean_object* l_zGame__wDraw_history__on__turn___rarg(lean_object*, lean_object*);
-LEAN_EXPORT lean_object* l_zGame__World__wDraw_world__after__fst(lean_object*, lean_object*);
-LEAN_EXPORT lean_object* l_zGame__wDraw_state__on__turn___rarg___boxed(lean_object*, lean_object*);
+LEAN_EXPORT lean_object* l_Game__World_world__after__fst___elambda__1___rarg(lean_object*, lean_object*, lean_object*, lean_object*);
+LEAN_EXPORT lean_object* l_zGame__World_snd__strat__deconditioned___rarg___boxed(lean_object*, lean_object*, lean_object*, lean_object*, lean_object*, lean_object*);
 LEAN_EXPORT lean_object* l_fst__strat__deconditioned___rarg___boxed(lean_object*, lean_object*, lean_object*, lean_object*, lean_object*);
 LEAN_EXPORT lean_object* l_snd__strat__deconditioned(lean_object*, lean_object*);
+LEAN_EXPORT lean_object* l_Game__World_world__after__fst___elambda__2(lean_object*, lean_object*);
 LEAN_EXPORT lean_object* l_snd__strat__deconditioned___rarg___boxed(lean_object*, lean_object*, lean_object*, lean_object*, lean_object*);
+LEAN_EXPORT lean_object* l_Game__World_world__after__fst(lean_object*, lean_object*);
+LEAN_EXPORT lean_object* l_Game__World_world__after__preHist___elambda__2___rarg(lean_object*, lean_object*, lean_object*, lean_object*);
+LEAN_EXPORT lean_object* l_zGame__World_snd__strat__conditioned(lean_object*, lean_object*);
+LEAN_EXPORT lean_object* l_zGame__World_snd__strat__deconditioned___rarg(lean_object*, lean_object*, lean_object*, lean_object*, lean_object*, lean_object*);
+LEAN_EXPORT lean_object* l_zGame_history__on__turn___rarg___boxed(lean_object*, lean_object*);
 uint8_t lean_nat_dec_eq(lean_object*, lean_object*);
 lean_object* l_History__on__turn___rarg(lean_object*, lean_object*, lean_object*, lean_object*);
+LEAN_EXPORT lean_object* l_Game__World_world__after__preHist(lean_object*, lean_object*);
 lean_object* lean_nat_sub(lean_object*, lean_object*);
+LEAN_EXPORT lean_object* l_zGame__World_snd__strat__conditioned___rarg___boxed(lean_object*, lean_object*, lean_object*, lean_object*, lean_object*);
 LEAN_EXPORT lean_object* l_snd__strat__deconditioned___rarg(lean_object*, lean_object*, lean_object*, lean_object*, lean_object*);
-LEAN_EXPORT lean_object* l_zGame__wDraw_state__on__turn(lean_object*, lean_object*);
-LEAN_EXPORT lean_object* l_Game__World__wDraw_world__after__preHist(lean_object*, lean_object*);
-LEAN_EXPORT lean_object* l_Game__World__wDraw_world__after__preHist___rarg(lean_object*, lean_object*);
+LEAN_EXPORT lean_object* l_zGame_history__on__turn___rarg(lean_object*, lean_object*);
 LEAN_EXPORT lean_object* l_instDecidableEqListNil(lean_object*);
 LEAN_EXPORT lean_object* l___private_Games_gameLib_Conditioning_0__History__on__turn_match__1_splitter___rarg(lean_object*, lean_object*, lean_object*);
+LEAN_EXPORT lean_object* l_zGame__World_world__after__fst(lean_object*, lean_object*);
 lean_object* l_List_redLength___rarg(lean_object*);
 lean_object* lean_nat_add(lean_object*, lean_object*);
-LEAN_EXPORT lean_object* l_zGame__wDraw_history__on__turn(lean_object*, lean_object*);
-LEAN_EXPORT lean_object* l_Game__World__wDraw_world__after__fst___rarg(lean_object*, lean_object*);
+LEAN_EXPORT lean_object* l_Game__World_world__after__fst___elambda__1(lean_object*, lean_object*);
+LEAN_EXPORT lean_object* l_zGame__World_snd__strat__conditioned___rarg(lean_object*, lean_object*, lean_object*, lean_object*, lean_object*);
+LEAN_EXPORT lean_object* l_zGame_state__on__turn___rarg___boxed(lean_object*, lean_object*);
 LEAN_EXPORT lean_object* l_fst__strat__deconditioned___rarg(lean_object*, lean_object*, lean_object*, lean_object*, lean_object*);
 lean_object* l_List_toArrayAux___rarg(lean_object*, lean_object*);
-LEAN_EXPORT lean_object* l_Game__World__wDraw_world__after__fst___rarg(lean_object* x_1, lean_object* x_2) {
+LEAN_EXPORT lean_object* l_zGame_state__on__turn(lean_object*, lean_object*);
+LEAN_EXPORT lean_object* l_Game__World_world__after__fst___elambda__1___rarg(lean_object* x_1, lean_object* x_2, lean_object* x_3, lean_object* x_4) {
 _start:
 {
-uint8_t x_3; 
-x_3 = !lean_is_exclusive(x_1);
-if (x_3 == 0)
-{
-lean_object* x_4; lean_object* x_5; lean_object* x_6; lean_object* x_7; 
-x_4 = lean_ctor_get(x_1, 0);
-x_5 = lean_ctor_get(x_1, 1);
-x_6 = lean_box(0);
+lean_object* x_5; lean_object* x_6; 
+x_5 = lean_ctor_get(x_1, 2);
 lean_inc(x_5);
-x_7 = lean_apply_3(x_5, x_4, x_6, x_2);
-lean_ctor_set(x_1, 0, x_7);
-return x_1;
-}
-else
-{
-lean_object* x_8; lean_object* x_9; lean_object* x_10; lean_object* x_11; lean_object* x_12; lean_object* x_13; 
-x_8 = lean_ctor_get(x_1, 0);
-x_9 = lean_ctor_get(x_1, 1);
-x_10 = lean_ctor_get(x_1, 2);
-lean_inc(x_10);
-lean_inc(x_9);
-lean_inc(x_8);
 lean_dec(x_1);
-x_11 = lean_box(0);
-lean_inc(x_9);
-x_12 = lean_apply_3(x_9, x_8, x_11, x_2);
-x_13 = lean_alloc_ctor(0, 3, 0);
-lean_ctor_set(x_13, 0, x_12);
-lean_ctor_set(x_13, 1, x_9);
-lean_ctor_set(x_13, 2, x_10);
-return x_13;
+x_6 = lean_apply_3(x_5, x_2, x_3, x_4);
+return x_6;
 }
 }
-}
-LEAN_EXPORT lean_object* l_Game__World__wDraw_world__after__fst(lean_object* x_1, lean_object* x_2) {
+LEAN_EXPORT lean_object* l_Game__World_world__after__fst___elambda__1(lean_object* x_1, lean_object* x_2) {
 _start:
 {
 lean_object* x_3; 
-x_3 = lean_alloc_closure((void*)(l_Game__World__wDraw_world__after__fst___rarg), 2, 0);
+x_3 = lean_alloc_closure((void*)(l_Game__World_world__after__fst___elambda__1___rarg), 4, 0);
+return x_3;
+}
+}
+LEAN_EXPORT lean_object* l_Game__World_world__after__fst___elambda__2___rarg(lean_object* x_1, lean_object* x_2, lean_object* x_3, lean_object* x_4) {
+_start:
+{
+lean_object* x_5; lean_object* x_6; 
+x_5 = lean_ctor_get(x_1, 1);
+lean_inc(x_5);
+lean_dec(x_1);
+x_6 = lean_apply_3(x_5, x_2, x_3, x_4);
+return x_6;
+}
+}
+LEAN_EXPORT lean_object* l_Game__World_world__after__fst___elambda__2(lean_object* x_1, lean_object* x_2) {
+_start:
+{
+lean_object* x_3; 
+x_3 = lean_alloc_closure((void*)(l_Game__World_world__after__fst___elambda__2___rarg), 4, 0);
+return x_3;
+}
+}
+LEAN_EXPORT lean_object* l_Game__World_world__after__fst___rarg(lean_object* x_1, lean_object* x_2) {
+_start:
+{
+lean_object* x_3; lean_object* x_4; lean_object* x_5; lean_object* x_6; lean_object* x_7; lean_object* x_8; 
+lean_inc(x_1);
+x_3 = lean_alloc_closure((void*)(l_Game__World_world__after__fst___elambda__2___rarg), 4, 1);
+lean_closure_set(x_3, 0, x_1);
+x_4 = lean_ctor_get(x_1, 0);
+lean_inc(x_4);
+x_5 = lean_box(0);
+lean_inc(x_1);
+x_6 = l_Game__World_world__after__fst___elambda__2___rarg(x_1, x_4, x_5, x_2);
+x_7 = lean_alloc_closure((void*)(l_Game__World_world__after__fst___elambda__1___rarg), 4, 1);
+lean_closure_set(x_7, 0, x_1);
+x_8 = lean_alloc_ctor(0, 3, 0);
+lean_ctor_set(x_8, 0, x_6);
+lean_ctor_set(x_8, 1, x_3);
+lean_ctor_set(x_8, 2, x_7);
+return x_8;
+}
+}
+LEAN_EXPORT lean_object* l_Game__World_world__after__fst(lean_object* x_1, lean_object* x_2) {
+_start:
+{
+lean_object* x_3; 
+x_3 = lean_alloc_closure((void*)(l_Game__World_world__after__fst___rarg), 2, 0);
 return x_3;
 }
 }
@@ -139,7 +172,7 @@ x_6 = l_instDecidableEqListNil___rarg(x_5);
 if (x_6 == 0)
 {
 lean_object* x_7; lean_object* x_8; lean_object* x_9; lean_object* x_10; lean_object* x_11; lean_object* x_12; lean_object* x_13; lean_object* x_14; 
-x_7 = l_Game__World__wDraw_world__after__fst___rarg(x_3, x_2);
+x_7 = l_Game__World_world__after__fst___rarg(x_3, x_2);
 x_8 = lean_ctor_get(x_7, 0);
 lean_inc(x_8);
 lean_dec(x_7);
@@ -182,7 +215,7 @@ LEAN_EXPORT lean_object* l_snd__strat__deconditioned___rarg(lean_object* x_1, le
 _start:
 {
 lean_object* x_6; lean_object* x_7; lean_object* x_8; lean_object* x_9; lean_object* x_10; lean_object* x_11; lean_object* x_12; lean_object* x_13; 
-x_6 = l_Game__World__wDraw_world__after__fst___rarg(x_3, x_2);
+x_6 = l_Game__World_world__after__fst___rarg(x_3, x_2);
 x_7 = lean_ctor_get(x_6, 0);
 lean_inc(x_7);
 lean_dec(x_6);
@@ -213,7 +246,45 @@ lean_dec(x_4);
 return x_6;
 }
 }
-LEAN_EXPORT lean_object* l_Game__World__wDraw_world__after__preHist___rarg(lean_object* x_1, lean_object* x_2) {
+LEAN_EXPORT lean_object* l_Game__World_world__after__preHist___elambda__1___rarg(lean_object* x_1, lean_object* x_2, lean_object* x_3, lean_object* x_4) {
+_start:
+{
+lean_object* x_5; lean_object* x_6; 
+x_5 = lean_ctor_get(x_1, 2);
+lean_inc(x_5);
+lean_dec(x_1);
+x_6 = lean_apply_3(x_5, x_2, x_3, x_4);
+return x_6;
+}
+}
+LEAN_EXPORT lean_object* l_Game__World_world__after__preHist___elambda__1(lean_object* x_1, lean_object* x_2) {
+_start:
+{
+lean_object* x_3; 
+x_3 = lean_alloc_closure((void*)(l_Game__World_world__after__preHist___elambda__1___rarg), 4, 0);
+return x_3;
+}
+}
+LEAN_EXPORT lean_object* l_Game__World_world__after__preHist___elambda__2___rarg(lean_object* x_1, lean_object* x_2, lean_object* x_3, lean_object* x_4) {
+_start:
+{
+lean_object* x_5; lean_object* x_6; 
+x_5 = lean_ctor_get(x_1, 1);
+lean_inc(x_5);
+lean_dec(x_1);
+x_6 = lean_apply_3(x_5, x_2, x_3, x_4);
+return x_6;
+}
+}
+LEAN_EXPORT lean_object* l_Game__World_world__after__preHist___elambda__2(lean_object* x_1, lean_object* x_2) {
+_start:
+{
+lean_object* x_3; 
+x_3 = lean_alloc_closure((void*)(l_Game__World_world__after__preHist___elambda__2___rarg), 4, 0);
+return x_3;
+}
+}
+LEAN_EXPORT lean_object* l_Game__World_world__after__preHist___rarg(lean_object* x_1, lean_object* x_2) {
 _start:
 {
 if (lean_obj_tag(x_2) == 0)
@@ -222,65 +293,84 @@ return x_1;
 }
 else
 {
-lean_object* x_3; lean_object* x_4; uint8_t x_5; 
+lean_object* x_3; lean_object* x_4; lean_object* x_5; lean_object* x_6; lean_object* x_7; lean_object* x_8; lean_object* x_9; 
 x_3 = lean_ctor_get(x_2, 0);
 lean_inc(x_3);
 x_4 = lean_ctor_get(x_2, 1);
 lean_inc(x_4);
 lean_dec(x_2);
-x_5 = !lean_is_exclusive(x_1);
+lean_inc(x_1);
+x_5 = lean_alloc_closure((void*)(l_Game__World_world__after__preHist___elambda__2___rarg), 4, 1);
+lean_closure_set(x_5, 0, x_1);
+x_6 = lean_ctor_get(x_1, 0);
+lean_inc(x_6);
+lean_inc(x_1);
+x_7 = l_Game__World_world__after__preHist___elambda__2___rarg(x_1, x_6, x_4, x_3);
+x_8 = lean_alloc_closure((void*)(l_Game__World_world__after__preHist___elambda__1___rarg), 4, 1);
+lean_closure_set(x_8, 0, x_1);
+x_9 = lean_alloc_ctor(0, 3, 0);
+lean_ctor_set(x_9, 0, x_7);
+lean_ctor_set(x_9, 1, x_5);
+lean_ctor_set(x_9, 2, x_8);
+return x_9;
+}
+}
+}
+LEAN_EXPORT lean_object* l_Game__World_world__after__preHist(lean_object* x_1, lean_object* x_2) {
+_start:
+{
+lean_object* x_3; 
+x_3 = lean_alloc_closure((void*)(l_Game__World_world__after__preHist___rarg), 2, 0);
+return x_3;
+}
+}
+LEAN_EXPORT lean_object* l_zGame__World_world__after__fst___rarg(lean_object* x_1, lean_object* x_2, lean_object* x_3) {
+_start:
+{
+lean_object* x_4; uint8_t x_5; 
+lean_inc(x_1);
+x_4 = l_Game__World_world__after__fst___rarg(x_1, x_2);
+x_5 = !lean_is_exclusive(x_4);
 if (x_5 == 0)
 {
-lean_object* x_6; lean_object* x_7; lean_object* x_8; 
-x_6 = lean_ctor_get(x_1, 0);
-x_7 = lean_ctor_get(x_1, 1);
-lean_inc(x_7);
-x_8 = lean_apply_3(x_7, x_6, x_4, x_3);
-lean_ctor_set(x_1, 0, x_8);
-return x_1;
+lean_object* x_6; lean_object* x_7; lean_object* x_8; lean_object* x_9; 
+x_6 = lean_ctor_get(x_4, 2);
+lean_dec(x_6);
+x_7 = lean_ctor_get(x_4, 1);
+lean_dec(x_7);
+lean_inc(x_1);
+x_8 = lean_alloc_closure((void*)(l_Game__World_world__after__fst___elambda__2___rarg), 4, 1);
+lean_closure_set(x_8, 0, x_1);
+x_9 = lean_alloc_closure((void*)(l_Game__World_world__after__fst___elambda__1___rarg), 4, 1);
+lean_closure_set(x_9, 0, x_1);
+lean_ctor_set(x_4, 2, x_9);
+lean_ctor_set(x_4, 1, x_8);
+return x_4;
 }
 else
 {
-lean_object* x_9; lean_object* x_10; lean_object* x_11; lean_object* x_12; lean_object* x_13; 
-x_9 = lean_ctor_get(x_1, 0);
-x_10 = lean_ctor_get(x_1, 1);
-x_11 = lean_ctor_get(x_1, 2);
-lean_inc(x_11);
+lean_object* x_10; lean_object* x_11; lean_object* x_12; lean_object* x_13; 
+x_10 = lean_ctor_get(x_4, 0);
 lean_inc(x_10);
-lean_inc(x_9);
-lean_dec(x_1);
-lean_inc(x_10);
-x_12 = lean_apply_3(x_10, x_9, x_4, x_3);
+lean_dec(x_4);
+lean_inc(x_1);
+x_11 = lean_alloc_closure((void*)(l_Game__World_world__after__fst___elambda__2___rarg), 4, 1);
+lean_closure_set(x_11, 0, x_1);
+x_12 = lean_alloc_closure((void*)(l_Game__World_world__after__fst___elambda__1___rarg), 4, 1);
+lean_closure_set(x_12, 0, x_1);
 x_13 = lean_alloc_ctor(0, 3, 0);
-lean_ctor_set(x_13, 0, x_12);
-lean_ctor_set(x_13, 1, x_10);
-lean_ctor_set(x_13, 2, x_11);
+lean_ctor_set(x_13, 0, x_10);
+lean_ctor_set(x_13, 1, x_11);
+lean_ctor_set(x_13, 2, x_12);
 return x_13;
 }
 }
 }
-}
-LEAN_EXPORT lean_object* l_Game__World__wDraw_world__after__preHist(lean_object* x_1, lean_object* x_2) {
+LEAN_EXPORT lean_object* l_zGame__World_world__after__fst(lean_object* x_1, lean_object* x_2) {
 _start:
 {
 lean_object* x_3; 
-x_3 = lean_alloc_closure((void*)(l_Game__World__wDraw_world__after__preHist___rarg), 2, 0);
-return x_3;
-}
-}
-LEAN_EXPORT lean_object* l_zGame__World__wDraw_world__after__fst___rarg(lean_object* x_1, lean_object* x_2, lean_object* x_3) {
-_start:
-{
-lean_object* x_4; 
-x_4 = l_Game__World__wDraw_world__after__fst___rarg(x_1, x_2);
-return x_4;
-}
-}
-LEAN_EXPORT lean_object* l_zGame__World__wDraw_world__after__fst(lean_object* x_1, lean_object* x_2) {
-_start:
-{
-lean_object* x_3; 
-x_3 = lean_alloc_closure((void*)(l_zGame__World__wDraw_world__after__fst___rarg), 3, 0);
+x_3 = lean_alloc_closure((void*)(l_zGame__World_world__after__fst___rarg), 3, 0);
 return x_3;
 }
 }
@@ -324,7 +414,7 @@ lean_dec(x_1);
 return x_4;
 }
 }
-LEAN_EXPORT lean_object* l_zGame__wDraw_history__on__turn___rarg(lean_object* x_1, lean_object* x_2) {
+LEAN_EXPORT lean_object* l_zGame_history__on__turn___rarg(lean_object* x_1, lean_object* x_2) {
 _start:
 {
 lean_object* x_3; lean_object* x_4; lean_object* x_5; lean_object* x_6; lean_object* x_7; 
@@ -342,24 +432,24 @@ x_7 = l_History__on__turn___rarg(x_4, x_5, x_6, x_2);
 return x_7;
 }
 }
-LEAN_EXPORT lean_object* l_zGame__wDraw_history__on__turn(lean_object* x_1, lean_object* x_2) {
+LEAN_EXPORT lean_object* l_zGame_history__on__turn(lean_object* x_1, lean_object* x_2) {
 _start:
 {
 lean_object* x_3; 
-x_3 = lean_alloc_closure((void*)(l_zGame__wDraw_history__on__turn___rarg___boxed), 2, 0);
+x_3 = lean_alloc_closure((void*)(l_zGame_history__on__turn___rarg___boxed), 2, 0);
 return x_3;
 }
 }
-LEAN_EXPORT lean_object* l_zGame__wDraw_history__on__turn___rarg___boxed(lean_object* x_1, lean_object* x_2) {
+LEAN_EXPORT lean_object* l_zGame_history__on__turn___rarg___boxed(lean_object* x_1, lean_object* x_2) {
 _start:
 {
 lean_object* x_3; 
-x_3 = l_zGame__wDraw_history__on__turn___rarg(x_1, x_2);
+x_3 = l_zGame_history__on__turn___rarg(x_1, x_2);
 lean_dec(x_2);
 return x_3;
 }
 }
-LEAN_EXPORT lean_object* l_zGame__wDraw_state__on__turn___rarg(lean_object* x_1, lean_object* x_2) {
+LEAN_EXPORT lean_object* l_zGame_state__on__turn___rarg(lean_object* x_1, lean_object* x_2) {
 _start:
 {
 lean_object* x_3; uint8_t x_4; 
@@ -371,7 +461,7 @@ lean_object* x_5; lean_object* x_6; lean_object* x_7; lean_object* x_8; uint8_t 
 x_5 = lean_unsigned_to_nat(1u);
 x_6 = lean_nat_sub(x_2, x_5);
 lean_inc(x_1);
-x_7 = l_zGame__wDraw_history__on__turn___rarg(x_1, x_6);
+x_7 = l_zGame_history__on__turn___rarg(x_1, x_6);
 x_8 = lean_nat_add(x_6, x_5);
 lean_dec(x_6);
 x_9 = l_instDecidablePredNatTurn__fst(x_8);
@@ -428,24 +518,24 @@ return x_23;
 }
 }
 }
-LEAN_EXPORT lean_object* l_zGame__wDraw_state__on__turn(lean_object* x_1, lean_object* x_2) {
+LEAN_EXPORT lean_object* l_zGame_state__on__turn(lean_object* x_1, lean_object* x_2) {
 _start:
 {
 lean_object* x_3; 
-x_3 = lean_alloc_closure((void*)(l_zGame__wDraw_state__on__turn___rarg___boxed), 2, 0);
+x_3 = lean_alloc_closure((void*)(l_zGame_state__on__turn___rarg___boxed), 2, 0);
 return x_3;
 }
 }
-LEAN_EXPORT lean_object* l_zGame__wDraw_state__on__turn___rarg___boxed(lean_object* x_1, lean_object* x_2) {
+LEAN_EXPORT lean_object* l_zGame_state__on__turn___rarg___boxed(lean_object* x_1, lean_object* x_2) {
 _start:
 {
 lean_object* x_3; 
-x_3 = l_zGame__wDraw_state__on__turn___rarg(x_1, x_2);
+x_3 = l_zGame_state__on__turn___rarg(x_1, x_2);
 lean_dec(x_2);
 return x_3;
 }
 }
-LEAN_EXPORT lean_object* l_zGame__World__wDraw_snd__strat__conditioned___rarg(lean_object* x_1, lean_object* x_2, lean_object* x_3, lean_object* x_4, lean_object* x_5) {
+LEAN_EXPORT lean_object* l_zGame__World_snd__strat__conditioned___rarg(lean_object* x_1, lean_object* x_2, lean_object* x_3, lean_object* x_4, lean_object* x_5) {
 _start:
 {
 lean_object* x_6; lean_object* x_7; lean_object* x_8; lean_object* x_9; lean_object* x_10; 
@@ -461,21 +551,68 @@ x_10 = lean_apply_2(x_1, x_6, x_9);
 return x_10;
 }
 }
-LEAN_EXPORT lean_object* l_zGame__World__wDraw_snd__strat__conditioned(lean_object* x_1, lean_object* x_2) {
+LEAN_EXPORT lean_object* l_zGame__World_snd__strat__conditioned(lean_object* x_1, lean_object* x_2) {
 _start:
 {
 lean_object* x_3; 
-x_3 = lean_alloc_closure((void*)(l_zGame__World__wDraw_snd__strat__conditioned___rarg___boxed), 5, 0);
+x_3 = lean_alloc_closure((void*)(l_zGame__World_snd__strat__conditioned___rarg___boxed), 5, 0);
 return x_3;
 }
 }
-LEAN_EXPORT lean_object* l_zGame__World__wDraw_snd__strat__conditioned___rarg___boxed(lean_object* x_1, lean_object* x_2, lean_object* x_3, lean_object* x_4, lean_object* x_5) {
+LEAN_EXPORT lean_object* l_zGame__World_snd__strat__conditioned___rarg___boxed(lean_object* x_1, lean_object* x_2, lean_object* x_3, lean_object* x_4, lean_object* x_5) {
 _start:
 {
 lean_object* x_6; 
-x_6 = l_zGame__World__wDraw_snd__strat__conditioned___rarg(x_1, x_2, x_3, x_4, x_5);
+x_6 = l_zGame__World_snd__strat__conditioned___rarg(x_1, x_2, x_3, x_4, x_5);
 lean_dec(x_4);
 return x_6;
+}
+}
+LEAN_EXPORT lean_object* l_zGame__World_snd__strat__deconditioned___rarg(lean_object* x_1, lean_object* x_2, lean_object* x_3, lean_object* x_4, lean_object* x_5, lean_object* x_6) {
+_start:
+{
+uint8_t x_7; 
+x_7 = l_instDecidableEqListNil___rarg(x_6);
+if (x_7 == 0)
+{
+lean_object* x_8; lean_object* x_9; lean_object* x_10; lean_object* x_11; lean_object* x_12; lean_object* x_13; lean_object* x_14; lean_object* x_15; 
+x_8 = l_zGame__World_world__after__fst___rarg(x_3, x_2, lean_box(0));
+x_9 = lean_ctor_get(x_8, 0);
+lean_inc(x_9);
+lean_dec(x_8);
+x_10 = l_List_redLength___rarg(x_6);
+x_11 = lean_mk_empty_array_with_capacity(x_10);
+lean_dec(x_10);
+x_12 = l_List_toArrayAux___rarg(x_6, x_11);
+x_13 = lean_array_pop(x_12);
+x_14 = lean_array_to_list(lean_box(0), x_13);
+x_15 = lean_apply_2(x_1, x_9, x_14);
+return x_15;
+}
+else
+{
+lean_dec(x_6);
+lean_dec(x_3);
+lean_dec(x_1);
+return x_2;
+}
+}
+}
+LEAN_EXPORT lean_object* l_zGame__World_snd__strat__deconditioned(lean_object* x_1, lean_object* x_2) {
+_start:
+{
+lean_object* x_3; 
+x_3 = lean_alloc_closure((void*)(l_zGame__World_snd__strat__deconditioned___rarg___boxed), 6, 0);
+return x_3;
+}
+}
+LEAN_EXPORT lean_object* l_zGame__World_snd__strat__deconditioned___rarg___boxed(lean_object* x_1, lean_object* x_2, lean_object* x_3, lean_object* x_4, lean_object* x_5, lean_object* x_6) {
+_start:
+{
+lean_object* x_7; 
+x_7 = l_zGame__World_snd__strat__deconditioned___rarg(x_1, x_2, x_3, x_4, x_5, x_6);
+lean_dec(x_5);
+return x_7;
 }
 }
 lean_object* initialize_Init(uint8_t builtin, lean_object*);
