Games/gameLib/Conditioning_wDraw.lean
@@ -9,57 +9,64 @@ import Games.gameLib.Termination
 
 
 
-def Game_World.world_after_fst {α β : Type u} (g : Game_World α β)
-  (fst_act : β) : Game_World α β := -- act not required to be legal
+def Game_World_wDraw.world_after_fst {α β : Type u} (g : Game_World_wDraw α β)
+  (fst_act : β) : Game_World_wDraw α β := -- act not required to be legal
   {g with init_game_state := g.fst_transition g.init_game_state [] fst_act }
 
 
 @[simp]
-lemma Game_World.world_after_fst_init {α β : Type u} (g : Game_World α β)
+lemma Game_World_wDraw.world_after_fst_init {α β : Type u} (g : Game_World_wDraw α β)
   (fst_act : β) : (g.world_after_fst fst_act).init_game_state = g.fst_transition g.init_game_state [] fst_act :=
   by rfl
 
 @[simp]
-lemma Game_World.world_after_fst_fst_legal {α β : Type u} (g : Game_World α β)
+lemma Game_World_wDraw.world_after_fst_fst_legal {α β : Type u} (g : Game_World_wDraw α β)
   (fst_act : β) : (g.world_after_fst fst_act).fst_legal = g.fst_legal :=
   by rfl
 
 @[simp]
-lemma Game_World.world_after_fst_snd_legal {α β : Type u} (g : Game_World α β)
+lemma Game_World_wDraw.world_after_fst_snd_legal {α β : Type u} (g : Game_World_wDraw α β)
   (fst_act : β) : (g.world_after_fst fst_act).snd_legal = g.snd_legal :=
   by rfl
 
 @[simp]
-lemma Game_World.world_after_fst_fst_win_states {α β : Type u} (g : Game_World α β)
+lemma Game_World_wDraw.world_after_fst_fst_win_states {α β : Type u} (g : Game_World_wDraw α β)
   (fst_act : β) : (g.world_after_fst fst_act).fst_win_states = g.fst_win_states :=
   by rfl
 
 
 @[simp]
-lemma Game_World.world_after_fst_snd_win_states {α β : Type u} (g : Game_World α β)
+lemma Game_World_wDraw.world_after_fst_snd_win_states {α β : Type u} (g : Game_World_wDraw α β)
   (fst_act : β) : (g.world_after_fst fst_act).snd_win_states = g.snd_win_states :=
   by rfl
 
 @[simp]
-lemma Game_World.world_after_fst_fst_transition {α β : Type u} (g : Game_World α β)
+lemma Game_World_wDraw.world_after_fst_draw_states {α β : Type u} (g : Game_World_wDraw α β)
+  (fst_act : β) : (g.world_after_fst fst_act).draw_states = g.draw_states :=
+  by rfl
+
+@[simp]
+lemma Game_World_wDraw.world_after_fst_fst_transition {α β : Type u} (g : Game_World_wDraw α β)
   (fst_act : β) : (g.world_after_fst fst_act).fst_transition = g.fst_transition :=
   by rfl
 
 @[simp]
-lemma Game_World.world_after_fst_snd_transition {α β : Type u} (g : Game_World α β)
+lemma Game_World_wDraw.world_after_fst_snd_transition {α β : Type u} (g : Game_World_wDraw α β)
   (fst_act : β) : (g.world_after_fst fst_act).snd_transition = g.snd_transition :=
   by rfl
 
 
 
+
 -- # Coherent end
 
-structure Game_World.coherent_end_aux
-  (g : Game_World α β) (f_strat s_strat : Strategy α β) (t : ℕ) : Prop where
+structure Game_World_wDraw.coherent_end_aux
+  (g : Game_World_wDraw α β) (f_strat s_strat : Strategy α β) (t : ℕ) : Prop where
   f : g.fst_win_states (g.state_on_turn f_strat s_strat t) → g.fst_win_states (g.state_on_turn f_strat s_strat (t+1))
   s : g.snd_win_states (g.state_on_turn f_strat s_strat t) → g.snd_win_states (g.state_on_turn f_strat s_strat (t+1))
+  d : g.draw_states (g.state_on_turn f_strat s_strat t) → g.draw_states (g.state_on_turn f_strat s_strat (t+1))
 
-def Game_World.coherent_end (g : Game_World α β) : Prop :=
+def Game_World_wDraw.coherent_end (g : Game_World_wDraw α β) : Prop :=
   ∀ f_strat s_strat : Strategy α β, ∀ t : ℕ, g.coherent_end_aux f_strat s_strat t
 
 
@@ -76,10 +83,10 @@ and is also explain by playing dummy vals, in a a priori impossible initial stat
 def law_nonprohibitive (law : α → List β → β → Prop) : Prop :=
   ∀ ini : α, ∀ hist : List β, ∃ act : β, law ini hist act
 
-def Game_World.playable (g : Game_World α β) : Prop :=
+def Game_World_wDraw.playable (g : Game_World_wDraw α β) : Prop :=
   law_nonprohibitive g.fst_legal ∧ law_nonprohibitive g.snd_legal
 
-lemma Game_World.playable_has_strat (g : Game_World α β)
+lemma Game_World_wDraw.playable_has_strat (g : Game_World_wDraw α β)
   (hg : g.playable) :
   ∃ f_strat : Strategy α β , ∃ s_strat : Strategy α β,
   Strategy_legal_fst g.init_game_state g.fst_legal f_strat s_strat ∧
@@ -91,49 +98,55 @@ lemma Game_World.playable_has_strat (g : Game_World α β)
   constructor
   · intro t _
     set hist := (History_on_turn g.init_game_state
-    (fun ini hist => Classical.choose (_ : ∃ act, Game_World.fst_legal g ini hist act))
-    (fun ini hist => Classical.choose (_ : ∃ act, Game_World.snd_legal g ini hist act)) t)
+    (fun ini hist => Classical.choose (_ : ∃ act, Game_World.fst_legal g.toGame_World ini hist act))
+    (fun ini hist => Classical.choose (_ : ∃ act, Game_World.snd_legal g.toGame_World ini hist act)) t)
     have pf := Classical.choose_spec (hg.1 g.init_game_state hist)
     apply pf
   · intro t _
     set hist := (History_on_turn g.init_game_state
-    (fun ini hist => Classical.choose (_ : ∃ act, Game_World.fst_legal g ini hist act))
-    (fun ini hist => Classical.choose (_ : ∃ act, Game_World.snd_legal g ini hist act)) t)
+    (fun ini hist => Classical.choose (_ : ∃ act, Game_World.fst_legal g.toGame_World ini hist act))
+    (fun ini hist => Classical.choose (_ : ∃ act, Game_World.snd_legal g.toGame_World ini hist act)) t)
     have ps:= Classical.choose_spec (hg.2 g.init_game_state hist)
     apply ps
 
 
 
--- # Easy termination
 
-
-inductive Game_World.has_WL (g : Game_World α β) : Prop where
-| wf : g.is_fst_win → g.has_WL
-| ws : g.is_snd_win → g.has_WL
-
-
-lemma Game_World.has_WL_init_end
-  (g : Game_World α β)
+lemma Game_World_wDraw.has_WLD_init_end
+  (g : Game_World_wDraw α β)
   (hg : g.playable)
   (P : Prop)
   (hp : P)
-  (h : (P ∧ (¬ g.snd_win_states g.init_game_state)) → g.has_WL) :
-  g.has_WL :=
+  (h : (P ∧ ((¬ g.draw_states g.init_game_state) ∧ (¬ g.snd_win_states g.init_game_state))) → g.has_WLD) :
+  g.has_WLD :=
   by
   obtain ⟨fs,ss,_,_⟩ := g.playable_has_strat hg
-  by_cases q2 : g.snd_win_states g.init_game_state
-  · apply Game_World.has_WL.ws
+  by_cases q1 : g.draw_states g.init_game_state
+  · apply Game_World_wDraw.has_WLD.d
+    right
     use fs
     intro _ _ _
     use 0
     constructor
     · decide
     · constructor
-      · apply q2
-      · intro t no
+      · dsimp [Game_wDraw.state_on_turn]
+        exact q1
+      · intro n no
         contradiction
-  · exact h ⟨hp, q2⟩
-
+  · by_cases q2 : g.snd_win_states g.init_game_state
+    · apply Game_World_wDraw.has_WLD.ws
+      use fs
+      intro _ _ _
+      use 0
+      constructor
+      · decide
+      · constructor
+        · dsimp [Game_wDraw.state_on_turn]
+          exact q2
+        · intro n no
+          contradiction
+    · exact h ⟨hp, q1, q2⟩
 
 
 
@@ -141,19 +154,19 @@ lemma Game_World.has_WL_init_end
 
 -- # zGame
 
-structure zGame_World (α β : Type _) extends Game_World α β where
-  f_legal_careless : careless toGame_World.fst_legal toGame_World.fst_transition
-  s_legal_careless : careless toGame_World.snd_legal toGame_World.fst_transition
-  f_transition_careless : careless toGame_World.fst_transition toGame_World.fst_transition
-  s_transition_careless : careless toGame_World.snd_transition toGame_World.fst_transition
-  coherent : toGame_World.coherent_end
-  playable : toGame_World.playable
-  sym_trans : toGame_World.fst_transition = toGame_World.snd_transition
-  sym_legal : toGame_World.fst_legal = toGame_World.snd_legal
-  sym_win : toGame_World.fst_win_states = toGame_World.snd_win_states
+structure zGame_World_wDraw (α β : Type _) extends Game_World_wDraw α β where
+  f_legal_careless : careless toGame_World_wDraw.fst_legal toGame_World_wDraw.fst_transition
+  s_legal_careless : careless toGame_World_wDraw.snd_legal toGame_World_wDraw.fst_transition
+  f_transition_careless : careless toGame_World_wDraw.fst_transition toGame_World_wDraw.fst_transition
+  s_transition_careless : careless toGame_World_wDraw.snd_transition toGame_World_wDraw.fst_transition
+  coherent : toGame_World_wDraw.coherent_end
+  playable : toGame_World_wDraw.playable
+  sym_trans : toGame_World_wDraw.fst_transition = toGame_World_wDraw.snd_transition
+  sym_legal : toGame_World_wDraw.fst_legal = toGame_World_wDraw.snd_legal
+  sym_win : toGame_World_wDraw.fst_win_states = toGame_World_wDraw.snd_win_states
 
 
-structure zGame (α β : Type _) extends zGame_World α β where
+structure zGame_wDraw (α β : Type _) extends zGame_World_wDraw α β where
   /-- The first players strategy-/
   fst_strat : Strategy α β
   /-- The second players strategy-/
@@ -173,14 +186,14 @@ instance (l : List α): Decidable (l = []) :=
 
 
 
-def fst_strat_deconditioned (s_strat : Strategy α β) (f_act : β) (g : Game_World α β) : Strategy α β :=
+def fst_strat_deconditioned (s_strat : Strategy α β) (f_act : β) (g : Game_World_wDraw α β) : Strategy α β :=
   (fun _ hist => if hist = [] then f_act else s_strat (g.world_after_fst f_act).init_game_state (hist.dropLast))
 
-def snd_strat_deconditioned (f_strat : Strategy α β) (f_act : β) (g : Game_World α β) : Strategy α β :=
+def snd_strat_deconditioned (f_strat : Strategy α β) (f_act : β) (g : Game_World_wDraw α β) : Strategy α β :=
   (fun _ hist => f_strat (g.world_after_fst f_act).init_game_state (hist.dropLast))
 
-lemma Game_World.History_of_deconditioned
-  (g: Game_World α β)
+lemma Game_World_wDraw.History_of_deconditioned
+  (g: Game_World_wDraw α β)
   (fst_act: β)
   (f_strat s_strat : Strategy α β)
   (turn : ℕ):
@@ -202,7 +215,7 @@ lemma Game_World.History_of_deconditioned
       rw [List.cons_append, ← ih]
       congr
       dsimp at ih
-      rw [← Game_World.world_after_fst_init] at ih
+      rw [← Game_World_wDraw.world_after_fst_init] at ih
       rw [ih]
       rw [snd_strat_deconditioned, List.dropLast_concat]
     · rw [if_neg q, if_neg q] at *
@@ -212,20 +225,20 @@ lemma Game_World.History_of_deconditioned
       rw [List.cons_append, ← ih]
       congr
       dsimp [snd_strat_deconditioned] at ih
-      rw [← Game_World.world_after_fst_init] at ih
+      rw [← Game_World_wDraw.world_after_fst_init] at ih
       rw [ih]
       rw [List.dropLast_concat]
 
 
 
-def Game_World.transition_blind_fst (g : Game_World α β) : Prop :=
+def Game_World_wDraw.transition_blind_fst (g : Game_World_wDraw α β) : Prop :=
   ∀ f_strat s_strat: Strategy α β, ∀ fst_act : β, g.fst_legal g.init_game_state [] fst_act →
   let fst_strat := fst_strat_deconditioned s_strat fst_act g
   let snd_strat := snd_strat_deconditioned f_strat fst_act g
   ∀ turn : ℕ, ∀ act : β, g.snd_transition (g.world_after_fst fst_act).init_game_state (History_on_turn (g.world_after_fst fst_act).init_game_state f_strat s_strat turn) act
     = g.fst_transition g.init_game_state (History_on_turn g.init_game_state fst_strat snd_strat (turn + 1)) act
 
-def Game_World.transition_blind_snd (g : Game_World α β) : Prop :=
+def Game_World_wDraw.transition_blind_snd (g : Game_World_wDraw α β) : Prop :=
   ∀ f_strat s_strat: Strategy α β, ∀ fst_act : β, g.fst_legal g.init_game_state [] fst_act →
   let fst_strat := fst_strat_deconditioned s_strat fst_act g
   let snd_strat := snd_strat_deconditioned f_strat fst_act g
@@ -233,75 +246,75 @@ def Game_World.transition_blind_snd (g : Game_World α β) : Prop :=
     = g.snd_transition g.init_game_state (History_on_turn g.init_game_state fst_strat snd_strat (turn + 1)) act
 
 
-def Game_World.transition_blind (g : Game_World α β) : Prop :=
+def Game_World_wDraw.transition_blind (g : Game_World_wDraw α β) : Prop :=
  g.transition_blind_fst ∧ g.transition_blind_snd
 
 
-def Game_World.strong_transition_blind_fst (g : Game_World α β) : Prop :=
+def Game_World_wDraw.strong_transition_blind_fst (g : Game_World_wDraw α β) : Prop :=
   ∀ fst_act : β, g.fst_legal g.init_game_state [] fst_act →
   ∀ hist : List β, ∀ act : β, g.snd_transition (g.world_after_fst fst_act).init_game_state hist act
     = g.fst_transition g.init_game_state (hist ++ [fst_act]) act
 
-def Game_World.strong_transition_blind_snd (g : Game_World α β) : Prop :=
+def Game_World_wDraw.strong_transition_blind_snd (g : Game_World_wDraw α β) : Prop :=
   ∀ fst_act : β, g.fst_legal g.init_game_state [] fst_act →
   ∀ hist : List β, ∀ act : β, g.fst_transition (g.world_after_fst fst_act).init_game_state hist act
     = g.snd_transition g.init_game_state (hist ++ [fst_act]) act
 
 
-def Game_World.strong_transition_blind (g : Game_World α β) : Prop :=
+def Game_World_wDraw.strong_transition_blind (g : Game_World_wDraw α β) : Prop :=
  g.strong_transition_blind_fst ∧ g.strong_transition_blind_snd
 
-lemma Game_World.strong_transition_blind_toWeak (g : Game_World α β) :
+lemma Game_World_wDraw.strong_transition_blind_toWeak (g : Game_World_wDraw α β) :
   g.strong_transition_blind → g.transition_blind :=
   by
   rintro ⟨f_strong, s_strong⟩
   constructor
   · intro f_strat s_strat f_act f_act_leg fst_strat snd_strat t act
-    rw [Game_World.History_of_deconditioned]
+    rw [Game_World_wDraw.History_of_deconditioned]
     apply f_strong
     exact f_act_leg
   · intro f_strat s_strat f_act f_act_leg fst_strat snd_strat t act
-    rw [Game_World.History_of_deconditioned]
+    rw [Game_World_wDraw.History_of_deconditioned]
     apply s_strong
     exact f_act_leg
 
 
 
-def Game_World.world_after_preHist {α β : Type u} (g : Game_World α β)
-  (prehist : List β) : Game_World α β := -- act not required to be legal
+def Game_World_wDraw.world_after_preHist {α β : Type u} (g : Game_World_wDraw α β)
+  (prehist : List β) : Game_World_wDraw α β := -- act not required to be legal
   match prehist with
   | [] => g
   | last :: L => {g with init_game_state := g.fst_transition g.init_game_state L last}
 
 
 
-def Game_World.hyper_transition_blind_fst (g : Game_World α β) : Prop :=
+def Game_World_wDraw.hyper_transition_blind_fst (g : Game_World_wDraw α β) : Prop :=
   ∀ prehist : List β, Hist_legal g.fst_legal g.snd_legal g.init_game_state prehist →
   ∀ hist : List β, ∀ act : β, g.snd_transition (g.world_after_preHist prehist).init_game_state hist act
     = g.fst_transition g.init_game_state (hist ++ prehist) act
 
-def Game_World.hyper_transition_blind_snd (g : Game_World α β) : Prop :=
+def Game_World_wDraw.hyper_transition_blind_snd (g : Game_World_wDraw α β) : Prop :=
   ∀ prehist : List β, Hist_legal g.fst_legal g.snd_legal g.init_game_state prehist →
   ∀ hist : List β, ∀ act : β, g.fst_transition (g.world_after_preHist prehist).init_game_state hist act
     = g.snd_transition g.init_game_state (hist ++ prehist) act
 
 
-def Game_World.hyper_transition_blind (g : Game_World α β) : Prop :=
+def Game_World_wDraw.hyper_transition_blind (g : Game_World_wDraw α β) : Prop :=
  g.hyper_transition_blind_fst ∧ g.hyper_transition_blind_snd
 
 
-lemma Game_World.hyper_transition_blind_transition_eq (g : Game_World α β) :
+lemma Game_World_wDraw.hyper_transition_blind_transition_eq (g : Game_World_wDraw α β) :
   g.hyper_transition_blind → (g.fst_transition g.init_game_state = g.snd_transition g.init_game_state) :=
   by
   intro h
   have := h.2 [] (by apply Hist_legal.nil)
-  dsimp [Game_World.world_after_preHist] at this
+  dsimp [Game_World_wDraw.world_after_preHist] at this
   simp_rw [List.append_nil] at this
   apply funext₂
   exact this
 
 
-lemma Game_World.hyper_transition_blind_toStrong (g : Game_World α β) :
+lemma Game_World_wDraw.hyper_transition_blind_toStrong (g : Game_World_wDraw α β) :
   g.hyper_transition_blind → g.strong_transition_blind :=
   by
   rintro ⟨f_hyper, s_hyper⟩
@@ -313,7 +326,7 @@ lemma Game_World.hyper_transition_blind_toStrong (g : Game_World α β) :
         rw [if_pos (by decide)]
         exact f_leg
       · apply Hist_legal.nil
-    · dsimp [Game_World.world_after_fst, Game_World.world_after_preHist] at *
+    · dsimp [Game_World_wDraw.world_after_fst, Game_World_wDraw.world_after_preHist] at *
       exact f_hyper
   · intro f_act f_leg hist act
     specialize s_hyper [f_act] _ hist act
@@ -322,18 +335,18 @@ lemma Game_World.hyper_transition_blind_toStrong (g : Game_World α β) :
         rw [if_pos (by decide)]
         exact f_leg
       · apply Hist_legal.nil
-    · dsimp [Game_World.world_after_fst, Game_World.world_after_preHist] at *
+    · dsimp [Game_World_wDraw.world_after_fst, Game_World_wDraw.world_after_preHist] at *
       exact s_hyper
 
 @[simp]
-lemma Game_World.world_after_preHist_singleton {α β : Type u} (g : Game_World α β)
+lemma Game_World_wDraw.world_after_preHist_singleton {α β : Type u} (g : Game_World_wDraw α β)
   (act : β) : g.world_after_preHist [act] = g.world_after_fst act :=
   by
-  dsimp [Game_World.world_after_fst, Game_World.world_after_preHist]
+  dsimp [Game_World_wDraw.world_after_fst, Game_World_wDraw.world_after_preHist]
 
 
-lemma zGame_World.is_hyper_transition_blind (g : zGame_World α β) :
-  g.toGame_World.hyper_transition_blind :=
+lemma zGame_World_wDraw.is_hyper_transition_blind (g : zGame_World_wDraw α β) :
+  g.toGame_World_wDraw.hyper_transition_blind :=
   by
   constructor
   · intro prehist preh_leg hist act
@@ -341,12 +354,12 @@ lemma zGame_World.is_hyper_transition_blind (g : zGame_World α β) :
     have that := g.sym_trans
     match prehist with
     | [] =>
-        dsimp [Game_World.world_after_preHist]
+        dsimp [Game_World_wDraw.world_after_preHist]
         rw [List.append_nil, that]
     | x :: l =>
         specialize this (by apply List.noConfusion)
         rw [this, that]
-        dsimp [Game_World.world_after_preHist]
+        dsimp [Game_World_wDraw.world_after_preHist]
         nth_rewrite 1 [that]
         rfl
   · intro prehist preh_leg hist act
@@ -354,18 +367,18 @@ lemma zGame_World.is_hyper_transition_blind (g : zGame_World α β) :
     have that := g.sym_trans
     match prehist with
     | [] =>
-        dsimp [Game_World.world_after_preHist]
+        dsimp [Game_World_wDraw.world_after_preHist]
         rw [List.append_nil, that]
     | x :: l =>
         specialize this (by apply List.noConfusion)
         rw [this, that]
-        dsimp [Game_World.world_after_preHist]
+        dsimp [Game_World_wDraw.world_after_preHist]
         nth_rewrite 1 [that]
         rfl
 
 
-lemma Game_World.State_of_deconditioned
-  (g: Game_World α β)
+lemma Game_World_wDraw.State_of_deconditioned
+  (g: Game_World_wDraw α β)
   (tb : g.transition_blind)
   (fst_act: β)
   (fst_act_legal: g.fst_legal g.init_game_state [] fst_act)
@@ -396,8 +409,8 @@ lemma Game_World.State_of_deconditioned
       clear this
       have := tb.2 f_strat s_strat fst_act fst_act_legal
       dsimp at this
-      specialize this t (f_strat (world_after_fst g fst_act).init_game_state (History_on_turn (world_after_fst g fst_act).init_game_state f_strat s_strat t))
-      rw [← Game_World.world_after_fst_init]
+      specialize this t (f_strat (world_after_fst g fst_act).toGame_World.init_game_state (History_on_turn (world_after_fst g fst_act).toGame_World.init_game_state f_strat s_strat t))
+      rw [← Game_World_wDraw.world_after_fst_init]
       rw [← this]
       clear this
       rfl
@@ -415,34 +428,34 @@ lemma Game_World.State_of_deconditioned
       clear this
       have := tb.1 f_strat s_strat fst_act fst_act_legal
       dsimp at this
-      specialize this t (s_strat (world_after_fst g fst_act).init_game_state (History_on_turn (Game_World.fst_transition g g.init_game_state [] fst_act) f_strat s_strat t))
-      rw [← Game_World.world_after_fst_init] at this
-      rw [← Game_World.world_after_fst_init]
+      specialize this t (s_strat (world_after_fst g fst_act).toGame_World.init_game_state (History_on_turn (Game_World.fst_transition g.toGame_World g.init_game_state [] fst_act) f_strat s_strat t))
+      rw [← Game_World_wDraw.world_after_fst_init] at this
+      rw [← Game_World_wDraw.world_after_fst_init]
       rw [← this]
 
 
-lemma zGame_World.State_of_deconditioned
-  (g: zGame_World α β)
+lemma zGame_World_wDraw.State_of_deconditioned
+  (g: zGame_World_wDraw α β)
   (fst_act: β)
   (fst_act_legal: g.fst_legal g.init_game_state [] fst_act)
   (f_strat s_strat : Strategy α β)
   (turn : ℕ):
-  let fst_strat := fst_strat_deconditioned s_strat fst_act g.toGame_World
-  let snd_strat := snd_strat_deconditioned f_strat fst_act g.toGame_World
+  let fst_strat := fst_strat_deconditioned s_strat fst_act g.toGame_World_wDraw
+  let snd_strat := snd_strat_deconditioned f_strat fst_act g.toGame_World_wDraw
   g.state_on_turn fst_strat snd_strat (turn + 1) =
   (g.world_after_fst fst_act).state_on_turn f_strat s_strat turn :=
   by
-  apply Game_World.State_of_deconditioned
-  · apply Game_World.strong_transition_blind_toWeak
-    apply Game_World.hyper_transition_blind_toStrong
-    apply zGame_World.is_hyper_transition_blind
+  apply Game_World_wDraw.State_of_deconditioned
+  · apply Game_World_wDraw.strong_transition_blind_toWeak
+    apply Game_World_wDraw.hyper_transition_blind_toStrong
+    apply zGame_World_wDraw.is_hyper_transition_blind
   · exact fst_act_legal
 
 
 
-def zGame_World.world_after_fst {α β : Type u} (g : zGame_World α β)
-  (fst_act : β) (fst_act_legal: g.fst_legal g.init_game_state [] fst_act) : zGame_World α β :=
-  {(g.toGame_World.world_after_fst fst_act) with
+def zGame_World_wDraw.world_after_fst {α β : Type u} (g : zGame_World_wDraw α β)
+  (fst_act : β) (fst_act_legal: g.fst_legal g.init_game_state [] fst_act) : zGame_World_wDraw α β :=
+  {(g.toGame_World_wDraw.world_after_fst fst_act) with
       f_legal_careless := by dsimp ; apply g.f_legal_careless
       s_legal_careless := by dsimp ; apply g.s_legal_careless
       f_transition_careless := by dsimp ; apply g.f_transition_careless
@@ -455,21 +468,28 @@ def zGame_World.world_after_fst {α β : Type u} (g : zGame_World α β)
                   constructor
                   · intro fws
                     dsimp at *
-                    have := g.State_of_deconditioned fst_act fst_act_legal f_strat s_strat
-                    dsimp [Game_World.world_after_fst] at this
-                    rw [← this] at *
-                    clear this
-                    have := (g.coherent (fst_strat_deconditioned s_strat fst_act g.toGame_World) (snd_strat_deconditioned f_strat fst_act g.toGame_World) (t+1)).f
+                    rw [Game_World_wDraw.state_on_turn_toGame_World] at *
+                    dsimp at *
+                    rw [← Game_World_wDraw.state_on_turn_toGame_World] at *
+                    rw [← g.State_of_deconditioned fst_act fst_act_legal f_strat s_strat] at *
+                    have := (g.coherent (fst_strat_deconditioned s_strat fst_act g.toGame_World_wDraw) (snd_strat_deconditioned f_strat fst_act g.toGame_World_wDraw) (t+1)).f
                     exact this fws
                   · intro fws
                     dsimp at *
-                    have := g.State_of_deconditioned fst_act fst_act_legal f_strat s_strat
-                    dsimp [Game_World.world_after_fst] at this
-                    rw [← this] at *
-                    clear this
-                    have := (g.coherent (fst_strat_deconditioned s_strat fst_act g.toGame_World) (snd_strat_deconditioned f_strat fst_act g.toGame_World) (t+1)).s
+                    rw [Game_World_wDraw.state_on_turn_toGame_World] at *
+                    dsimp at *
+                    rw [← Game_World_wDraw.state_on_turn_toGame_World] at *
+                    rw [← g.State_of_deconditioned fst_act fst_act_legal f_strat s_strat] at *
+                    have := (g.coherent (fst_strat_deconditioned s_strat fst_act g.toGame_World_wDraw) (snd_strat_deconditioned f_strat fst_act g.toGame_World_wDraw) (t+1)).s
                     exact this fws
-
+                  · intro fws
+                    dsimp at *
+                    rw [Game_World_wDraw.state_on_turn_toGame_World] at *
+                    dsimp at *
+                    rw [← Game_World_wDraw.state_on_turn_toGame_World] at *
+                    rw [← g.State_of_deconditioned fst_act fst_act_legal f_strat s_strat] at *
+                    have := (g.coherent (fst_strat_deconditioned s_strat fst_act g.toGame_World_wDraw) (snd_strat_deconditioned f_strat fst_act g.toGame_World_wDraw) (t+1)).d
+                    exact this fws
       playable := by
                   constructor
                   · dsimp
@@ -479,9 +499,7 @@ def zGame_World.world_after_fst {α β : Type u} (g : zGame_World α β)
                   }
 
 
-
-
-lemma zGame_World.world_after_fst_init (g : zGame_World α β)
+lemma zGame_World_wDraw.world_after_fst_init (g : zGame_World_wDraw α β)
   (fst_act : β) (fst_act_legal: g.fst_legal g.init_game_state [] fst_act) :
   (g.world_after_fst fst_act fst_act_legal).init_game_state = g.fst_transition g.init_game_state [] fst_act :=
   by
@@ -489,38 +507,44 @@ lemma zGame_World.world_after_fst_init (g : zGame_World α β)
 
 
 @[simp]
-lemma zGame_World.world_after_fst_fst_legal {α β : Type u} (g : zGame_World α β)
+lemma zGame_World_wDraw.world_after_fst_fst_legal {α β : Type u} (g : zGame_World_wDraw α β)
   (fst_act : β) (fst_act_legal: g.fst_legal g.init_game_state [] fst_act) :
   (g.world_after_fst fst_act fst_act_legal).fst_legal = g.fst_legal :=
   by rfl
 
 @[simp]
-lemma zGame_World.world_after_fst_snd_legal {α β : Type u} (g : zGame_World α β)
+lemma zGame_World_wDraw.world_after_fst_snd_legal {α β : Type u} (g : zGame_World_wDraw α β)
   (fst_act : β) (fst_act_legal: g.fst_legal g.init_game_state [] fst_act) :
   (g.world_after_fst fst_act fst_act_legal).snd_legal = g.snd_legal :=
   by rfl
 
 @[simp]
-lemma zGame_World.world_after_fst_fst_win_states {α β : Type u} (g : zGame_World α β)
+lemma zGame_World_wDraw.world_after_fst_fst_win_states {α β : Type u} (g : zGame_World_wDraw α β)
   (fst_act : β) (fst_act_legal: g.fst_legal g.init_game_state [] fst_act) :
   (g.world_after_fst fst_act fst_act_legal).fst_win_states = g.fst_win_states :=
   by rfl
 
 
 @[simp]
-lemma zGame_World.world_after_fst_snd_win_states {α β : Type u} (g : zGame_World α β)
+lemma zGame_World_wDraw.world_after_fst_snd_win_states {α β : Type u} (g : zGame_World_wDraw α β)
   (fst_act : β) (fst_act_legal: g.fst_legal g.init_game_state [] fst_act) :
   (g.world_after_fst fst_act fst_act_legal).snd_win_states = g.snd_win_states :=
   by rfl
 
 @[simp]
-lemma zGame_World.world_after_fst_fst_transition {α β : Type u} (g : zGame_World α β)
+lemma zGame_World_wDraw.world_after_fst_draw_states {α β : Type u} (g : zGame_World_wDraw α β)
+  (fst_act : β) (fst_act_legal: g.fst_legal g.init_game_state [] fst_act) :
+  (g.world_after_fst fst_act fst_act_legal).draw_states = g.draw_states :=
+  by rfl
+
+@[simp]
+lemma zGame_World_wDraw.world_after_fst_fst_transition {α β : Type u} (g : zGame_World_wDraw α β)
   (fst_act : β) (fst_act_legal: g.fst_legal g.init_game_state [] fst_act) :
   (g.world_after_fst fst_act fst_act_legal).fst_transition = g.fst_transition :=
   by rfl
 
 @[simp]
-lemma zGame_World.world_after_fst_snd_transition {α β : Type u} (g : zGame_World α β)
+lemma zGame_World_wDraw.world_after_fst_snd_transition {α β : Type u} (g : zGame_World_wDraw α β)
   (fst_act : β) (fst_act_legal: g.fst_legal g.init_game_state [] fst_act) :
   (g.world_after_fst fst_act fst_act_legal).snd_transition = g.snd_transition :=
   by rfl
@@ -530,28 +554,28 @@ lemma zGame_World.world_after_fst_snd_transition {α β : Type u} (g : zGame_Wor
 -- # Careless strat
 
 
-def Game_World.Strategy_blind_fst (strat : Strategy α β) (g : Game_World α β) : Prop :=
+def Game_World_wDraw.Strategy_blind_fst (strat : Strategy α β) (g : Game_World_wDraw α β) : Prop :=
   ∀ s_strat: Strategy α β,
   let fst_act := strat g.init_game_state []
   ∀ turn : ℕ, strat (g.world_after_fst fst_act).init_game_state (History_on_turn (g.world_after_fst fst_act).init_game_state s_strat strat turn)
     = strat g.init_game_state (History_on_turn g.init_game_state strat s_strat (turn + 1))
 
 
-def Game_World.Strategy_blind_snd (strat : Strategy α β) (g : Game_World α β) : Prop :=
+def Game_World_wDraw.Strategy_blind_snd (strat : Strategy α β) (g : Game_World_wDraw α β) : Prop :=
   ∀ f_strat: Strategy α β,
   let fst_act := f_strat g.init_game_state []
   ∀ turn : ℕ, strat (g.world_after_fst fst_act).init_game_state (History_on_turn (g.world_after_fst fst_act).init_game_state strat f_strat turn)
     = strat g.init_game_state (History_on_turn g.init_game_state f_strat strat (turn + 1))
 
-def Game_World.Strategy_blind (strat : Strategy α β) (g : Game_World α β) : Prop :=
+def Game_World_wDraw.Strategy_blind (strat : Strategy α β) (g : Game_World_wDraw α β) : Prop :=
   g.Strategy_blind_fst strat ∧ g.Strategy_blind_snd strat
 
-def Game_World.strong_Strategy_blind (strat : Strategy α β) (g : Game_World α β) : Prop :=
+def Game_World_wDraw.strong_Strategy_blind (strat : Strategy α β) (g : Game_World_wDraw α β) : Prop :=
   ∀ fst_act : β, g.fst_legal g.init_game_state [] fst_act →
   ∀ hist : List β, strat (g.world_after_fst fst_act).init_game_state hist
     = strat g.init_game_state (hist ++ [fst_act])
 
-lemma Game_World.world_after_fst_History_blind (g : Game_World α β)
+lemma Game_World_wDraw.world_after_fst_History_blind (g : Game_World_wDraw α β)
   (f_strat s_strat : Strategy α β) (turn : ℕ)
   (hf : g.Strategy_blind_fst f_strat) (hs : g.Strategy_blind_snd s_strat)
   :
@@ -569,11 +593,11 @@ lemma Game_World.world_after_fst_History_blind (g : Game_World α β)
       rw [if_neg q]
       rw [← Turn_fst_not_step] at q
       rw [if_pos q]
-      rw [Game_World.world_after_fst_init] at *
+      rw [Game_World_wDraw.world_after_fst_init] at *
       rw [List.cons_append, ih]
       congr 1
       have := hs f_strat t
-      rw [← Game_World.world_after_fst_init, this]
+      rw [← Game_World_wDraw.world_after_fst_init, this]
       dsimp [History_on_turn]
       rw [if_pos q]
     · rw [if_neg q] at *
@@ -581,17 +605,17 @@ lemma Game_World.world_after_fst_History_blind (g : Game_World α β)
       rw [if_pos q]
       rw [← @not_not (Turn_fst (t + 1 + 1)), ← Turn_fst_not_step] at q
       rw [if_neg q]
-      rw [Game_World.world_after_fst_init] at *
+      rw [Game_World_wDraw.world_after_fst_init] at *
       rw [List.cons_append]
       congr 1
       have := hf s_strat t
-      rw [Game_World.world_after_fst_init] at this
+      rw [Game_World_wDraw.world_after_fst_init] at this
       rw [this]
       dsimp [History_on_turn]
       rw [if_neg q]
 
 
-lemma Game_World.world_after_fst_History_strong_blind (g : Game_World α β)
+lemma Game_World_wDraw.world_after_fst_History_strong_blind (g : Game_World_wDraw α β)
   (f_strat s_strat : Strategy α β) (turn : ℕ)
   (f_leg : Strategy_legal_fst g.init_game_state g.fst_legal f_strat s_strat)
   (hf : g.strong_Strategy_blind f_strat) (hs : g.strong_Strategy_blind s_strat)
@@ -607,20 +631,20 @@ lemma Game_World.world_after_fst_History_strong_blind (g : Game_World α β)
     by_cases q : Turn_fst (t+1)
     · rw [if_pos q]
       rw [List.cons_append, ih]
-      specialize hs (f_strat g.init_game_state []) (by apply f_leg 0 (by decide)) (History_on_turn (Game_World.fst_transition g g.init_game_state [] (f_strat g.init_game_state [])) s_strat f_strat t)
-      rw [← Game_World.world_after_fst_init] at hs
+      specialize hs (f_strat g.init_game_state []) (by apply f_leg 0 (by decide)) (History_on_turn (Game_World.fst_transition g.toGame_World g.init_game_state [] (f_strat g.init_game_state [])) s_strat f_strat t)
+      rw [← Game_World_wDraw.world_after_fst_init] at hs
       rw [hs, ih]
       rw [if_neg (show ¬ Turn_fst (Nat.succ t + 1) from (by rw [← Turn_fst_not_step]; exact q))]
     · rw [if_neg q]
       rw [List.cons_append, ih]
-      specialize hf (f_strat g.init_game_state []) (by apply f_leg 0 (by decide)) (History_on_turn (Game_World.fst_transition g g.init_game_state [] (f_strat g.init_game_state [])) s_strat f_strat t)
-      rw [← Game_World.world_after_fst_init] at hf
+      specialize hf (f_strat g.init_game_state []) (by apply f_leg 0 (by decide)) (History_on_turn (Game_World.fst_transition g.toGame_World g.init_game_state [] (f_strat g.init_game_state [])) s_strat f_strat t)
+      rw [← Game_World_wDraw.world_after_fst_init] at hf
       rw [hf, ih]
       rw [if_pos (show Turn_fst (Nat.succ t + 1) from (by rw [iff_not_comm.mp (Turn_fst_not_step (t+1))]; exact q))]
 
 
 -- might not be the case, because we have no carelessness of other strat
--- lemma Game_World.strong_Strategy_blind_toWeak (strat : Strategy α β) (g : Game_World α β)
+-- lemma Game_World_wDraw.strong_Strategy_blind_toWeak (strat : Strategy α β) (g : Game_World_wDraw α β)
 --   (f_leg : Strategy_legal_fst g.init_game_state g.fst_legal strat s_strat) :
 --   g.strong_Strategy_blind strat → g.Strategy_blind strat :=
 --   by
@@ -633,15 +657,15 @@ lemma Game_World.world_after_fst_History_strong_blind (g : Game_World α β)
 
 --#exit
 
-def Game_World.hyper_Strategy_blind
-  (strat : Strategy α β) (g : Game_World α β) : Prop :=
+def Game_World_wDraw.hyper_Strategy_blind
+  (strat : Strategy α β) (g : Game_World_wDraw α β) : Prop :=
   ∀ prehist : List β, Hist_legal g.fst_legal g.snd_legal g.init_game_state prehist →
   ∀ hist : List β, strat (g.world_after_preHist prehist).init_game_state hist
     = strat g.init_game_state (hist ++ prehist)
 
 
-lemma Game_World.hyper_Strategy_blind_toStrong
-  (strat : Strategy α β) (g : Game_World α β) :
+lemma Game_World_wDraw.hyper_Strategy_blind_toStrong
+  (strat : Strategy α β) (g : Game_World_wDraw α β) :
   g.hyper_Strategy_blind strat → g.strong_Strategy_blind strat :=
   by
   intro hyp
@@ -652,7 +676,7 @@ lemma Game_World.hyper_Strategy_blind_toStrong
       rw [if_pos (by decide)]
       exact f_leg
     · apply Hist_legal.nil
-  · dsimp [Game_World.world_after_fst, Game_World.world_after_preHist] at *
+  · dsimp [Game_World_wDraw.world_after_fst, Game_World_wDraw.world_after_preHist] at *
     exact hyp
 
 
@@ -660,14 +684,14 @@ lemma Game_World.hyper_Strategy_blind_toStrong
 
 -- # Blind law
 
-def Game_World.legal_blind_fst (g : Game_World α β) : Prop :=
+def Game_World_wDraw.legal_blind_fst (g : Game_World_wDraw α β) : Prop :=
   ∀ f_strat s_strat: Strategy α β, ∀ fst_act : β, g.fst_legal g.init_game_state [] fst_act →
   let fst_strat := fst_strat_deconditioned s_strat fst_act g
   let snd_strat := snd_strat_deconditioned f_strat fst_act g
   ∀ turn : ℕ, ∀ act : β, g.snd_legal (g.world_after_fst fst_act).init_game_state (History_on_turn (g.world_after_fst fst_act).init_game_state f_strat s_strat turn) act
     = g.fst_legal g.init_game_state (History_on_turn g.init_game_state fst_strat snd_strat (turn + 1)) act
 
-def Game_World.legal_blind_snd (g : Game_World α β) : Prop :=
+def Game_World_wDraw.legal_blind_snd (g : Game_World_wDraw α β) : Prop :=
   ∀ f_strat s_strat: Strategy α β, ∀ fst_act : β, g.fst_legal g.init_game_state [] fst_act →
   let fst_strat := fst_strat_deconditioned s_strat fst_act g
   let snd_strat := snd_strat_deconditioned f_strat fst_act g
@@ -675,68 +699,68 @@ def Game_World.legal_blind_snd (g : Game_World α β) : Prop :=
     = g.snd_legal g.init_game_state (History_on_turn g.init_game_state fst_strat snd_strat (turn + 1)) act
 
 
-def Game_World.legal_blind (g : Game_World α β) : Prop :=
+def Game_World_wDraw.legal_blind (g : Game_World_wDraw α β) : Prop :=
  g.legal_blind_fst ∧ g.legal_blind_snd
 
 
-def Game_World.strong_legal_blind_fst (g : Game_World α β) : Prop :=
+def Game_World_wDraw.strong_legal_blind_fst (g : Game_World_wDraw α β) : Prop :=
   ∀ fst_act : β, g.fst_legal g.init_game_state [] fst_act →
   ∀ hist : List β, ∀ act : β, g.snd_legal (g.world_after_fst fst_act).init_game_state hist act
     = g.fst_legal g.init_game_state (hist ++ [fst_act]) act
 
-def Game_World.strong_legal_blind_snd (g : Game_World α β) : Prop :=
+def Game_World_wDraw.strong_legal_blind_snd (g : Game_World_wDraw α β) : Prop :=
   ∀ fst_act : β, g.fst_legal g.init_game_state [] fst_act →
   ∀ hist : List β, ∀ act : β, g.fst_legal (g.world_after_fst fst_act).init_game_state hist act
     = g.snd_legal g.init_game_state (hist ++ [fst_act]) act
 
 
-def Game_World.strong_legal_blind (g : Game_World α β) : Prop :=
+def Game_World_wDraw.strong_legal_blind (g : Game_World_wDraw α β) : Prop :=
  g.strong_legal_blind_fst ∧ g.strong_legal_blind_snd
 
-lemma Game_World.strong_legal_blind_toWeak (g : Game_World α β) :
+lemma Game_World_wDraw.strong_legal_blind_toWeak (g : Game_World_wDraw α β) :
   g.strong_legal_blind → g.legal_blind :=
   by
   rintro ⟨f_strong, s_strong⟩
   constructor
   · intro f_strat s_strat f_act f_act_leg fst_strat snd_strat t act
-    rw [Game_World.History_of_deconditioned]
+    rw [Game_World_wDraw.History_of_deconditioned]
     apply f_strong
     exact f_act_leg
   · intro f_strat s_strat f_act f_act_leg fst_strat snd_strat t act
-    rw [Game_World.History_of_deconditioned]
+    rw [Game_World_wDraw.History_of_deconditioned]
     apply s_strong
     exact f_act_leg
 
 
 
 
-def Game_World.hyper_legal_blind_fst (g : Game_World α β) : Prop :=
+def Game_World_wDraw.hyper_legal_blind_fst (g : Game_World_wDraw α β) : Prop :=
   ∀ prehist : List β, Hist_legal g.fst_legal g.snd_legal g.init_game_state prehist →
   ∀ hist : List β, ∀ act : β, g.snd_legal (g.world_after_preHist prehist).init_game_state hist act
     = g.fst_legal g.init_game_state (hist ++ prehist) act
 
-def Game_World.hyper_legal_blind_snd (g : Game_World α β) : Prop :=
+def Game_World_wDraw.hyper_legal_blind_snd (g : Game_World_wDraw α β) : Prop :=
   ∀ prehist : List β, Hist_legal g.fst_legal g.snd_legal g.init_game_state prehist →
   ∀ hist : List β, ∀ act : β, g.fst_legal (g.world_after_preHist prehist).init_game_state hist act
     = g.snd_legal g.init_game_state (hist ++ prehist) act
 
 
-def Game_World.hyper_legal_blind (g : Game_World α β) : Prop :=
+def Game_World_wDraw.hyper_legal_blind (g : Game_World_wDraw α β) : Prop :=
  g.hyper_legal_blind_fst ∧ g.hyper_legal_blind_snd
 
 
-lemma Game_World.hyper_legal_blind_legal_eq (g : Game_World α β) :
+lemma Game_World_wDraw.hyper_legal_blind_legal_eq (g : Game_World_wDraw α β) :
   g.hyper_legal_blind → (g.fst_legal g.init_game_state = g.snd_legal g.init_game_state) :=
   by
   intro h
   have := h.2 [] (by apply Hist_legal.nil)
-  dsimp [Game_World.world_after_preHist] at this
+  dsimp [Game_World_wDraw.world_after_preHist] at this
   simp_rw [List.append_nil] at this
   apply funext₂
   exact this
 
 
-lemma Game_World.hyper_legal_blind_toStrong (g : Game_World α β) :
+lemma Game_World_wDraw.hyper_legal_blind_toStrong (g : Game_World_wDraw α β) :
   g.hyper_legal_blind → g.strong_legal_blind :=
   by
   rintro ⟨f_hyper, s_hyper⟩
@@ -748,7 +772,7 @@ lemma Game_World.hyper_legal_blind_toStrong (g : Game_World α β) :
         rw [if_pos (by decide)]
         exact f_leg
       · apply Hist_legal.nil
-    · dsimp [Game_World.world_after_fst, Game_World.world_after_preHist] at *
+    · dsimp [Game_World_wDraw.world_after_fst, Game_World_wDraw.world_after_preHist] at *
       exact f_hyper
   · intro f_act f_leg hist act
     specialize s_hyper [f_act] _ hist act
@@ -757,12 +781,12 @@ lemma Game_World.hyper_legal_blind_toStrong (g : Game_World α β) :
         rw [if_pos (by decide)]
         exact f_leg
       · apply Hist_legal.nil
-    · dsimp [Game_World.world_after_fst, Game_World.world_after_preHist] at *
+    · dsimp [Game_World_wDraw.world_after_fst, Game_World_wDraw.world_after_preHist] at *
       exact s_hyper
 
 
-lemma zGame_World.is_hyper_legal_blind (g : zGame_World α β) :
-  g.toGame_World.hyper_legal_blind :=
+lemma zGame_World_wDraw.is_hyper_legal_blind (g : zGame_World_wDraw α β) :
+  g.toGame_World_wDraw.hyper_legal_blind :=
   by
   constructor
   · intro prehist preh_leg hist act
@@ -770,28 +794,28 @@ lemma zGame_World.is_hyper_legal_blind (g : zGame_World α β) :
     have that := g.sym_legal
     match prehist with
     | [] =>
-        dsimp [Game_World.world_after_preHist]
+        dsimp [Game_World_wDraw.world_after_preHist]
         rw [List.append_nil, that]
     | x :: l =>
         specialize this (by apply List.noConfusion)
         rw [this, that]
-        dsimp [Game_World.world_after_preHist]
+        dsimp [Game_World_wDraw.world_after_preHist]
   · intro prehist preh_leg hist act
     have := g.s_legal_careless g.init_game_state hist prehist
     have that := g.sym_legal
     match prehist with
     | [] =>
-        dsimp [Game_World.world_after_preHist]
+        dsimp [Game_World_wDraw.world_after_preHist]
         rw [List.append_nil, that]
     | x :: l =>
         specialize this (by apply List.noConfusion)
         rw [this, that]
-        dsimp [Game_World.world_after_preHist]
+        dsimp [Game_World_wDraw.world_after_preHist]
 
 
 
-lemma Game_World.fst_legal_deconditioned
-  (g: Game_World α β)
+lemma Game_World_wDraw.fst_legal_deconditioned
+  (g: Game_World_wDraw α β)
   (fst_act: β)
   (fst_act_legal: g.fst_legal g.init_game_state [] fst_act)
   (f_strat s_strat : Strategy α β)
@@ -807,7 +831,7 @@ lemma Game_World.fst_legal_deconditioned
   · dsimp [History_on_turn, fst_strat_deconditioned]
     rw [if_pos (by rfl)]
     exact fst_act_legal
-  · rw [← b, Game_World.History_of_deconditioned]
+  · rw [← b, Game_World_wDraw.History_of_deconditioned]
     · dsimp [History_on_turn, fst_strat_deconditioned]
       rw [if_neg (by apply List.append_ne_nil_of_ne_nil_right ; exact List.cons_ne_nil fst_act [])]
       rw [List.dropLast_concat]
@@ -817,8 +841,8 @@ lemma Game_World.fst_legal_deconditioned
     · exact fst_act_legal
 
 
-lemma Game_World.snd_legal_deconditioned
-  (g: Game_World α β)
+lemma Game_World_wDraw.snd_legal_deconditioned
+  (g: Game_World_wDraw α β)
   (fst_act: β)
   (fst_act_legal: g.fst_legal g.init_game_state [] fst_act)
   (f_strat s_strat : Strategy α β)
@@ -832,7 +856,7 @@ lemma Game_World.snd_legal_deconditioned
   intro fst_strat snd_strat t tf
   cases' t with t
   · contradiction
-  · rw [← b, Game_World.History_of_deconditioned]
+  · rw [← b, Game_World_wDraw.History_of_deconditioned]
     · dsimp [History_on_turn, snd_strat_deconditioned]
       rw [List.dropLast_concat]
       apply f_leg
@@ -841,11 +865,11 @@ lemma Game_World.snd_legal_deconditioned
     · exact fst_act_legal
 
 
-def zGame.history_on_turn {α β : Type u} (g : zGame α β) : ℕ → List β :=
+def zGame_wDraw.history_on_turn {α β : Type u} (g : zGame_wDraw α β) : ℕ → List β :=
   History_on_turn g.init_game_state g.fst_strat g.snd_strat
 
 
-def zGame.state_on_turn {α β : Type u} (g : zGame α β) : ℕ → α
+def zGame_wDraw.state_on_turn {α β : Type u} (g : zGame_wDraw α β) : ℕ → α
 | 0 => g.init_game_state
 | n+1 => let h := g.history_on_turn n
          if Turn_fst (n+1)
@@ -860,41 +884,119 @@ def zGame.state_on_turn {α β : Type u} (g : zGame α β) : ℕ → α
 
 
 
-def zGame.fst_win  {α β : Type _} (g : zGame α β) : Prop :=
+def zGame_wDraw.fst_win  {α β : Type _} (g : zGame_wDraw α β) : Prop :=
   ∃ turn : ℕ, Turn_fst turn ∧ g.fst_win_states (g.state_on_turn turn) ∧
     (∀ t < turn, g.state_on_turn_neutral g.fst_strat g.snd_strat t)
 
 
-def zGame.snd_win  {α β : Type u} (g : zGame α β) : Prop :=
+def zGame_wDraw.snd_win  {α β : Type u} (g : zGame_wDraw α β) : Prop :=
   ∃ turn : ℕ, Turn_snd turn  ∧ g.snd_win_states (g.state_on_turn turn) ∧
     (∀ t < turn, g.state_on_turn_neutral g.fst_strat g.snd_strat t)
 
 
+def zGame_wDraw.fst_draw {α β : Type u} (g : zGame_wDraw α β) : Prop :=
+  ∃ turn : ℕ, Turn_fst turn  ∧ g.draw_states (g.state_on_turn turn) ∧
+    (∀ t < turn, g.state_on_turn_neutral g.fst_strat g.snd_strat t)
 
-def zGame_World.is_fst_win  {α β : Type u} (g : zGame_World α β) : Prop :=
+
+def zGame_wDraw.snd_draw {α β : Type u} (g : zGame_wDraw α β) : Prop :=
+  ∃ turn : ℕ, Turn_snd turn  ∧ g.draw_states (g.state_on_turn turn) ∧
+    (∀ t < turn, g.state_on_turn_neutral g.fst_strat g.snd_strat t)
+
+
+def zGame_wDraw.draw {α β : Type u} (g : zGame_wDraw α β) : Prop :=
+  g.fst_draw ∨ g.snd_draw
+
+
+def zGame_World_wDraw.is_fst_win  {α β : Type u} (g : zGame_World_wDraw α β) : Prop :=
   ∃ ws : Strategy α β, --g.Strategy_blind_fst ws ∧
   ∀ snd_s : Strategy α β, --g.Strategy_blind_fst snd_s →
    (ws_leg : Strategy_legal_fst g.init_game_state g.fst_legal ws snd_s) →
    (snd_leg : Strategy_legal_snd g.init_game_state g.snd_legal ws snd_s) →
-  ({g with fst_strat := ws, fst_lawful := ws_leg, snd_strat := snd_s, snd_lawful := snd_leg} : Game α β).fst_win
+  ({g with fst_strat := ws, fst_lawful := ws_leg, snd_strat := snd_s, snd_lawful := snd_leg} : Game_wDraw α β).fst_win
 
 
-def zGame_World.is_snd_win  {α β : Type u} (g : zGame_World α β) : Prop :=
+def zGame_World_wDraw.is_snd_win  {α β : Type u} (g : zGame_World_wDraw α β) : Prop :=
   ∃ ws : Strategy α β, -- g.Strategy_blind_snd ws ∧
   ∀ fst_s : Strategy α β, --g.Strategy_blind_snd fst_s →
    (ws_leg : Strategy_legal_snd g.init_game_state g.snd_legal fst_s ws) →
    (fst_leg : Strategy_legal_fst g.init_game_state g.fst_legal fst_s ws) →
-  ({g with fst_strat := fst_s, fst_lawful := fst_leg, snd_strat := ws, snd_lawful := ws_leg} : Game α β).snd_win
+  ({g with fst_strat := fst_s, fst_lawful := fst_leg, snd_strat := ws, snd_lawful := ws_leg} : Game_wDraw α β).snd_win
+
+def zGame_World_wDraw.is_fst_draw  {α β : Type u} (g : zGame_World_wDraw α β) : Prop :=
+  ∃ ws : Strategy α β, -- g.Strategy_blind_fst ws ∧
+  ∀ snd_s : Strategy α β, -- g.Strategy_blind_fst snd_s →
+   (ws_leg : Strategy_legal_fst g.init_game_state g.fst_legal ws snd_s) →
+   (snd_leg : Strategy_legal_snd g.init_game_state g.snd_legal ws snd_s) →
+  ({g with fst_strat := ws, fst_lawful := ws_leg, snd_strat := snd_s, snd_lawful := snd_leg} : Game_wDraw α β).fst_draw
+
+
+def zGame_World_wDraw.is_snd_draw  {α β : Type u} (g : zGame_World_wDraw α β) : Prop :=
+  ∃ ws : Strategy α β,-- g.Strategy_blind_snd ws ∧
+  ∀ fst_s : Strategy α β, -- g.Strategy_blind_snd fst_s →
+   (ws_leg : Strategy_legal_snd g.init_game_state g.snd_legal fst_s ws) →
+   (fst_leg : Strategy_legal_fst g.init_game_state g.fst_legal fst_s ws) →
+  ({g with fst_strat := fst_s, fst_lawful := fst_leg, snd_strat := ws, snd_lawful := ws_leg} : Game_wDraw α β).snd_draw
 
 
 
-inductive zGame_World.has_WL (g : zGame_World α β) : Prop where
+def zGame_wDraw.is_draw {α β : Type u} (g : zGame_wDraw α β) : Prop :=
+  g.is_fst_draw ∨ g.is_snd_draw
+
+
+
+inductive zGame_World_wDraw.has_WLD (g : zGame_World_wDraw α β) : Prop where
+| wf : g.is_fst_win → g.has_WLD
+| ws : g.is_snd_win → g.has_WLD
+| d : g.is_draw → g.has_WLD
+
+
+lemma zGame_World_wDraw.has_WLD_init_end
+  (g : zGame_World_wDraw α β)
+  (P : Prop)
+  (hp : P)
+  (h : (P ∧ ((¬ g.draw_states g.init_game_state) ∧ (¬ g.snd_win_states g.init_game_state))) → g.has_WLD) :
+  g.has_WLD :=
+  by
+  obtain ⟨fs,ss,_,_⟩ := g.playable_has_strat g.playable
+  by_cases q1 : g.draw_states g.init_game_state
+  · apply zGame_World_wDraw.has_WLD.d
+    right
+    use fs
+    intro _ _ _
+    use 0
+    constructor
+    · decide
+    · constructor
+      · dsimp [Game_wDraw.state_on_turn]
+        exact q1
+      · intro n no
+        contradiction
+  · by_cases q2 : g.snd_win_states g.init_game_state
+    · apply zGame_World_wDraw.has_WLD.ws
+      use fs
+      intro _ _ _
+      use 0
+      constructor
+      · decide
+      · constructor
+        · apply q2
+        · intro t no
+          contradiction
+    · exact h ⟨hp, q1, q2⟩
+
+
+
+-- # Easy termination
+
+
+inductive zGame_World_wDraw.has_WL (g : zGame_World_wDraw α β) : Prop where
 | wf : g.is_fst_win → g.has_WL
 | ws : g.is_snd_win → g.has_WL
 
 
-lemma zGame_World.has_WL_init_end
-  (g : zGame_World α β)
+lemma zGame_World_wDraw.has_WL_init_end
+  (g : zGame_World_wDraw α β)
   (P : Prop)
   (hp : P)
   (h : (P ∧ (¬ g.snd_win_states g.init_game_state)) → g.has_WL) :
@@ -902,7 +1004,7 @@ lemma zGame_World.has_WL_init_end
   by
   obtain ⟨fs,ss,_,_⟩ := g.playable_has_strat g.playable
   by_cases q2 : g.snd_win_states g.init_game_state
-  · apply zGame_World.has_WL.ws
+  · apply zGame_World_wDraw.has_WL.ws
     use fs
     intro _ _ _
     use 0
@@ -918,13 +1020,13 @@ lemma zGame_World.has_WL_init_end
 
 -- # More conditioining
 
-def zGame_World.snd_strat_conditioned (f_strat : Strategy α β) (f_act : β) (g : zGame_World α β) : Strategy α β :=
+def zGame_World_wDraw.snd_strat_conditioned (f_strat : Strategy α β) (f_act : β) (g : zGame_World_wDraw α β) : Strategy α β :=
   fun _ hist => f_strat g.init_game_state (hist ++ [f_act])
 
 open Classical
 
 noncomputable
-def zGame_World.fst_strat_conditioned [Inhabited β] (g : zGame_World α β)
+def zGame_World_wDraw.fst_strat_conditioned [Inhabited β] (g : zGame_World_wDraw α β)
   (f_strat : (h : List β) → (hne : h ≠ []) → (hl : g.fst_legal g.init_game_state [] (h.getLast hne)) → Strategy α β)
   : Strategy α β :=
   fun (_ : α) hist  =>
@@ -935,8 +1037,8 @@ def zGame_World.fst_strat_conditioned [Inhabited β] (g : zGame_World α β)
          then (f_strat hist hh H) (g.fst_transition g.init_game_state [] f_act) hist.dropLast -- is it ? since ref to history in current game
          else default
 
-lemma zGame_World.history_on_turn_conditioned
-  [Inhabited β] (g : zGame_World α β) (fst_s: Strategy α β)
+lemma zGame_World_wDraw.history_on_turn_conditioned
+  [Inhabited β] (g : zGame_World_wDraw α β) (fst_s: Strategy α β)
   (f_strat : (h : List β) → (hne : h ≠ []) → (hl : g.fst_legal g.init_game_state [] (h.getLast hne)) → Strategy α β)
   (h_f_strat : ∀ h H: List β, (hne : h ≠ []) → (Hne : H ≠ []) →
       (hl : g.fst_legal g.init_game_state [] (h.getLast hne)) → (Hl : g.fst_legal g.init_game_state [] (H.getLast Hne)) →
@@ -950,28 +1052,28 @@ lemma zGame_World.history_on_turn_conditioned
   by
   intro f_act t
   induction' t with t ih
-  · dsimp [Game_World.history_on_turn, History_on_turn]
+  · dsimp [Game_World_wDraw.history_on_turn, History_on_turn]
     rw [if_pos (by decide)]
-  · dsimp [Game_World.history_on_turn, History_on_turn]
+  · dsimp [Game_World_wDraw.history_on_turn, History_on_turn]
     by_cases q : Turn_fst (Nat.succ t + 1)
     · rw [if_pos q]
       rw [iff_not_comm.mp (Turn_fst_not_step (t+1))] at q
       rw [if_neg q,if_neg q]
-      dsimp [zGame_World.snd_strat_conditioned]
-      unfold Game_World.history_on_turn at ih
+      dsimp [zGame_World_wDraw.snd_strat_conditioned]
+      unfold Game_World_wDraw.history_on_turn at ih
       rw [← ih]
       dsimp [History_on_turn]
       rw [if_neg q]
     · rw [if_neg q]
       rw [iff_not_comm.mp (Turn_fst_not_step (t+1)), not_not] at q
       rw [if_pos q, if_pos q]
-      dsimp [zGame_World.fst_strat_conditioned]
+      dsimp [zGame_World_wDraw.fst_strat_conditioned]
       rw [dif_neg (by apply List.cons_ne_nil)]
       have := History_on_turn_getLast_fst_act g.init_game_state fst_s (g.fst_strat_conditioned f_strat) (t)
       dsimp [History_on_turn] at this
       simp_rw [if_pos q] at this
       rw [dif_pos (by rw [this] ; apply f_act_leg)]
-      unfold Game_World.history_on_turn at ih
+      unfold Game_World_wDraw.history_on_turn at ih
       rw [← ih]
       have that : History_on_turn g.init_game_state fst_s (fst_strat_conditioned g f_strat) (t + 1) =
                   (fst_s g.init_game_state (History_on_turn g.init_game_state fst_s (fst_strat_conditioned g f_strat) t) ::
@@ -999,8 +1101,8 @@ lemma zGame_World.history_on_turn_conditioned
 
 
 
-lemma zGame_World.state_on_turn_conditioned
-  [Inhabited β] (g : zGame_World α β) (fst_s: Strategy α β)
+lemma zGame_World_wDraw.state_on_turn_conditioned
+  [Inhabited β] (g : zGame_World_wDraw α β) (fst_s: Strategy α β)
   (f_strat : (h : List β) → (hne : h ≠ []) → (hl : g.fst_legal g.init_game_state [] (h.getLast hne)) → Strategy α β)
   (h_f_strat : ∀ h H: List β, (hne : h ≠ []) → (Hne : H ≠ []) →
       (hl : g.fst_legal g.init_game_state [] (h.getLast hne)) → (Hl : g.fst_legal g.init_game_state [] (H.getLast Hne)) →
@@ -1014,17 +1116,17 @@ lemma zGame_World.state_on_turn_conditioned
   by
   intro f_act t
   cases' t with t
-  · dsimp [Game_World.state_on_turn]
+  · dsimp [Game_World_wDraw.state_on_turn]
     rw [if_pos (by decide)]
-    dsimp [Game_World.history_on_turn, History_on_turn, zGame_World.world_after_fst_init]
-  · dsimp [Game_World.state_on_turn]
+    dsimp [Game_World_wDraw.history_on_turn, History_on_turn, zGame_World_wDraw.world_after_fst_init]
+  · dsimp [Game_World_wDraw.state_on_turn]
     by_cases q : Turn_fst (t + 1 + 1)
     · rw [if_pos q]
       rw [iff_not_comm.mp (Turn_fst_not_step (t+1))] at q
       rw [if_neg q]
       rw [g.history_on_turn_conditioned fst_s f_strat h_f_strat f_act_leg]
       have := careless_singleton _ _ (g.f_transition_careless)
-      specialize this g.init_game_state ((Game_World.history_on_turn (world_after_fst g (fst_s g.init_game_state []) f_act_leg).toGame_World
+      specialize this g.init_game_state ((Game_World_wDraw.history_on_turn (world_after_fst g (fst_s g.init_game_state []) f_act_leg).toGame_World_wDraw
           (f_strat [fst_s g.init_game_state []] ((by apply List.cons_ne_nil) : [fst_s g.init_game_state []] ≠ []) f_act_leg)
           (snd_strat_conditioned fst_s (fst_s g.init_game_state []) g) t)) f_act
       simp_rw [this]
@@ -1037,7 +1139,7 @@ lemma zGame_World.state_on_turn_conditioned
       rw [if_pos q]
       rw [g.history_on_turn_conditioned fst_s f_strat h_f_strat f_act_leg]
       have := careless_singleton _ _ (g.s_transition_careless)
-      specialize this g.init_game_state ((Game_World.history_on_turn (world_after_fst g (fst_s g.init_game_state []) f_act_leg).toGame_World
+      specialize this g.init_game_state ((Game_World_wDraw.history_on_turn (world_after_fst g (fst_s g.init_game_state []) f_act_leg).toGame_World_wDraw
           (f_strat [fst_s g.init_game_state []] ((by apply List.cons_ne_nil) : [fst_s g.init_game_state []] ≠ []) f_act_leg)
           (snd_strat_conditioned fst_s (fst_s g.init_game_state []) g) t)) f_act
       simp_rw [this]
@@ -1049,7 +1151,7 @@ lemma zGame_World.state_on_turn_conditioned
       rw [List.dropLast_append_of_ne_nil _ (show [f_act] ≠ [] from by apply List.cons_ne_nil)]
       dsimp
       rw [List.append_nil]
-      have := h_f_strat ((Game_World.history_on_turn (world_after_fst g (fst_s g.init_game_state []) f_act_leg).toGame_World
+      have := h_f_strat ((Game_World_wDraw.history_on_turn (world_after_fst g (fst_s g.init_game_state []) f_act_leg).toGame_World_wDraw
             (f_strat [fst_s g.init_game_state []] ((by apply List.cons_ne_nil) : [fst_s g.init_game_state []] ≠ []) f_act_leg)
             (snd_strat_conditioned fst_s (fst_s g.init_game_state []) g) t ++
              [fst_s g.init_game_state []])) [f_act]
@@ -1064,8 +1166,8 @@ lemma zGame_World.state_on_turn_conditioned
 
 
 
-lemma zGame_World.conditioned_legal_fst
-  [Inhabited β] (g : zGame_World α β) (fst_s: Strategy α β)
+lemma zGame_World_wDraw.conditioned_legal_fst
+  [Inhabited β] (g : zGame_World_wDraw α β) (fst_s: Strategy α β)
   (f_strat : (h : List β) → (hne : h ≠ []) → (hl : g.fst_legal g.init_game_state [] (h.getLast hne)) → Strategy α β)
   (h_f_strat : ∀ h H: List β, (hne : h ≠ []) → (Hne : H ≠ []) →
       (hl : g.fst_legal g.init_game_state [] (h.getLast hne)) → (Hl : g.fst_legal g.init_game_state [] (H.getLast Hne)) →
@@ -1082,7 +1184,7 @@ lemma zGame_World.conditioned_legal_fst
     have hh := g.history_on_turn_conditioned fst_s f_strat h_f_strat f_act_leg t
     have hc := careless_singleton _ _ (g.f_legal_careless)
     specialize leg (t+1) (by rw [← Turn_snd_fst_step] ; exact ts)
-    unfold Game_World.history_on_turn at hh
+    unfold Game_World_wDraw.history_on_turn at hh
     rw [hh] at leg
     rw [hc] at leg
     dsimp [snd_strat_conditioned]
@@ -1095,7 +1197,7 @@ lemma zGame_World.conditioned_legal_fst
     · specialize leg (t) (by rw [Turn_snd_fst_step] ; exact tf)
       have hh := g.history_on_turn_conditioned fst_s f_strat h_f_strat f_act_leg t
       have hc := careless_singleton _ _ (g.f_legal_careless)
-      unfold Game_World.history_on_turn at hh
+      unfold Game_World_wDraw.history_on_turn at hh
       rw [hh, hc]
       dsimp [snd_strat_conditioned] at leg
       rw [g.sym_legal]
@@ -1104,8 +1206,8 @@ lemma zGame_World.conditioned_legal_fst
 
 
 
-lemma zGame_World.conditioned_legal_snd
-  [Inhabited β] (g : zGame_World α β) (fst_s: Strategy α β)
+lemma zGame_World_wDraw.conditioned_legal_snd
+  [Inhabited β] (g : zGame_World_wDraw α β) (fst_s: Strategy α β)
   (f_strat : (h : List β) → (hne : h ≠ []) → (hl : g.fst_legal g.init_game_state [] (h.getLast hne)) → Strategy α β)
   (h_f_strat : ∀ h H: List β, (hne : h ≠ []) → (Hne : H ≠ []) →
       (hl : g.fst_legal g.init_game_state [] (h.getLast hne)) → (Hl : g.fst_legal g.init_game_state [] (H.getLast Hne)) →
@@ -1122,7 +1224,7 @@ lemma zGame_World.conditioned_legal_snd
     have hh := g.history_on_turn_conditioned fst_s f_strat h_f_strat f_act_leg t
     have hc := careless_singleton _ _ (g.s_legal_careless)
     specialize leg (t+1) (by rw [← Turn_fst_snd_step] ; exact tf)
-    unfold Game_World.history_on_turn at hh
+    unfold Game_World_wDraw.history_on_turn at hh
     rw [hh] at leg
     rw [hc] at leg
     dsimp [snd_strat_conditioned]
@@ -1133,7 +1235,7 @@ lemma zGame_World.conditioned_legal_snd
     rw [List.dropLast_append_of_ne_nil _ (show [f_act] ≠ [] from by apply List.cons_ne_nil)] at leg
     dsimp at leg
     rw [List.append_nil] at leg
-    have := h_f_strat ((Game_World.history_on_turn (world_after_fst g (fst_s g.init_game_state []) f_act_leg).toGame_World
+    have := h_f_strat ((Game_World_wDraw.history_on_turn (world_after_fst g (fst_s g.init_game_state []) f_act_leg).toGame_World_wDraw
             (f_strat [fst_s g.init_game_state []] ((by apply List.cons_ne_nil) : [fst_s g.init_game_state []] ≠ []) f_act_leg)
             (snd_strat_conditioned fst_s (fst_s g.init_game_state []) g) t ++
              [fst_s g.init_game_state []])) [f_act]
@@ -1142,7 +1244,7 @@ lemma zGame_World.conditioned_legal_snd
              (by rw [List.getLast_append] ; apply f_act_leg)
              (by apply f_act_leg)
              (by rw [List.getLast_append] ; dsimp)
-    unfold Game_World.history_on_turn at this
+    unfold Game_World_wDraw.history_on_turn at this
     rw [this] at leg
     rw [List.getLast_append] at leg
     apply leg
@@ -1152,11 +1254,11 @@ lemma zGame_World.conditioned_legal_snd
     · have hh := g.history_on_turn_conditioned fst_s f_strat h_f_strat f_act_leg t
       have hc := careless_singleton _ _ (g.s_legal_careless)
       specialize leg (t) (by rw [Turn_fst_snd_step] ; exact ts)
-      unfold Game_World.history_on_turn at hh
+      unfold Game_World_wDraw.history_on_turn at hh
       rw [hh]
       rw [hc]
       rw [← g.sym_legal]
-      rw [zGame_World.world_after_fst_fst_legal] at leg
+      rw [zGame_World_wDraw.world_after_fst_fst_legal] at leg
       convert leg using 1
       dsimp [fst_strat_conditioned]
       rw [dif_neg (by apply List.append_ne_nil_of_ne_nil_right ; apply List.cons_ne_nil)]
@@ -1164,7 +1266,7 @@ lemma zGame_World.conditioned_legal_snd
       rw [List.dropLast_append_of_ne_nil _ (show [f_act] ≠ [] from by apply List.cons_ne_nil)]
       dsimp
       rw [List.append_nil]
-      have := h_f_strat ((Game_World.history_on_turn (world_after_fst g (fst_s g.init_game_state []) f_act_leg).toGame_World
+      have := h_f_strat ((Game_World_wDraw.history_on_turn (world_after_fst g (fst_s g.init_game_state []) f_act_leg).toGame_World_wDraw
               (f_strat [fst_s g.init_game_state []] ((by apply List.cons_ne_nil) : [fst_s g.init_game_state []] ≠ []) f_act_leg)
               (snd_strat_conditioned fst_s (fst_s g.init_game_state []) g) t ++
               [fst_s g.init_game_state []])) [f_act]
@@ -1173,15 +1275,15 @@ lemma zGame_World.conditioned_legal_snd
               (by rw [List.getLast_append] ; apply f_act_leg)
               (by apply f_act_leg)
               (by rw [List.getLast_append] ; dsimp)
-      unfold Game_World.history_on_turn at this
+      unfold Game_World_wDraw.history_on_turn at this
       rw [this]
       rw [List.getLast_append]
       rfl
 
 
 
-lemma zGame_World.conditioned_state_on_turn_neutral
-  [Inhabited β] (g : zGame_World α β) (fst_s: Strategy α β)
+lemma zGame_World_wDraw.conditioned_state_on_turn_neutral
+  [Inhabited β] (g : zGame_World_wDraw α β) (fst_s: Strategy α β)
   (f_strat : (h : List β) → (hne : h ≠ []) → (hl : g.fst_legal g.init_game_state [] (h.getLast hne)) → Strategy α β)
   (h_f_strat : ∀ h H: List β, (hne : h ≠ []) → (Hne : H ≠ []) →
       (hl : g.fst_legal g.init_game_state [] (h.getLast hne)) → (Hl : g.fst_legal g.init_game_state [] (H.getLast Hne)) →
@@ -1194,8 +1296,9 @@ lemma zGame_World.conditioned_state_on_turn_neutral
   (g.world_after_fst f_act f_act_leg).state_on_turn_neutral (f_strat [f_act] (List.cons_ne_nil f_act []) f_act_leg) (g.snd_strat_conditioned fst_s f_act) t:=
   by
   intro f_act t
-  dsimp [Game_World.state_on_turn_neutral]
+  dsimp [Game_World_wDraw.state_on_turn_neutral]
   rw [g.state_on_turn_conditioned fst_s f_strat h_f_strat f_act_leg]
+  congr 1
   by_cases q : Turn_fst t
   · rw [if_pos q]
     rw [Turn_fst_not_step] at q
@@ -1209,8 +1312,25 @@ lemma zGame_World.conditioned_state_on_turn_neutral
 
 
 
+
+--#exit
+
+-- lemma zGame_World_wDraw.conditioned_legal_fst' [Inhabited β] (f_strat fst_s: Strategy α β) (g : zGame_World_wDraw α β) :
+--   let ws := g.fst_strat_conditioned fst_s
+--   (f_leg : Strategy_legal_fst g.init_game_state g.fst_legal f_strat ws) →
+--   (ws_leg : Strategy_legal_snd g.init_game_state g.fst_legal f_strat ws) →
+--   let f_act := f_strat g.init_game_state []
+--   let f_act_leg := f_leg 0 (by decide)
+--   Strategy_legal_fst (g.world_after_fst f_act f_act_leg).init_game_state (g.world_after_fst f_act f_act_leg).fst_legal f_strat (g.snd_strat_conditioned f_strat f_act) :=
+--   by -- replace fst_act wih stuff
+--   sorry -- test on Zermelo first
+
+-- -- lemma zGame_World_wDraw.getLast_is_fst [Inhabited β] (g : zGame_World_wDraw α β)
+-- --   (f_strat s_strat: Strategy α β)
+-- --   (hist : List β) (hh : hist ≠ []) :
+
 lemma History_on_turn_eq_strats_snd
-  (g : zGame_World α β) (f_strat sSa aSb: Strategy α β)
+  (g : zGame_World_wDraw α β) (f_strat sSa aSb: Strategy α β)
   (h : ∀ t, Turn_snd (t+1) →  sSa g.init_game_state (History_on_turn g.init_game_state f_strat sSa (t)) =
           sSb g.init_game_state (History_on_turn g.init_game_state f_strat sSb (t))) :
   History_on_turn g.init_game_state f_strat sSa = History_on_turn g.init_game_state f_strat sSb :=
@@ -1226,7 +1346,7 @@ lemma History_on_turn_eq_strats_snd
 
 
 lemma Strategy_legal_fst_eq_strats_snd
-  (g : zGame_World α β) (f_strat sSa sSb: Strategy α β)
+  (g : zGame_World_wDraw α β) (f_strat sSa sSb: Strategy α β)
   (h : ∀ t, Turn_snd (t+1) → sSa g.init_game_state (History_on_turn g.init_game_state f_strat sSa (t)) =
           sSb g.init_game_state (History_on_turn g.init_game_state f_strat sSb (t)))
   (hl : Strategy_legal_fst g.init_game_state g.fst_legal f_strat sSa) :
@@ -1238,7 +1358,7 @@ lemma Strategy_legal_fst_eq_strats_snd
 
 
 lemma Strategy_legal_snd_eq_strats_snd
-  (g : zGame_World α β) (f_strat sSa sSb: Strategy α β)
+  (g : zGame_World_wDraw α β) (f_strat sSa sSb: Strategy α β)
   (h : ∀ t, Turn_snd (t+1) → sSa g.init_game_state (History_on_turn g.init_game_state f_strat sSa (t)) =
           sSb g.init_game_state (History_on_turn g.init_game_state f_strat sSb (t)))
   (hl : Strategy_legal_snd g.init_game_state g.snd_legal f_strat sSa) :
@@ -1252,36 +1372,37 @@ lemma Strategy_legal_snd_eq_strats_snd
 
 
 
-lemma Conditioning_win [Inhabited β] (g : zGame_World α β) (fst_s: Strategy α β)
+lemma Conditioning_win [Inhabited β] (g : zGame_World_wDraw α β) (fst_s: Strategy α β)
   (f_strat : (h : List β) → (hne : h ≠ []) → (hl : g.fst_legal g.init_game_state [] (h.getLast hne)) → Strategy α β)
   (h_f_strat : ∀ h H: List β, (hne : h ≠ []) → (Hne : H ≠ []) →
       (hl : g.fst_legal g.init_game_state [] (h.getLast hne)) → (Hl : g.fst_legal g.init_game_state [] (H.getLast Hne)) →
       h.getLast hne = H.getLast Hne →
       f_strat h hne hl = f_strat H Hne Hl)
   (f_act_leg : g.fst_legal g.init_game_state [] (fst_s g.init_game_state []))
-  (Leg_f : Strategy_legal_fst g.init_game_state g.fst_legal fst_s (zGame_World.fst_strat_conditioned g f_strat))
-  (Leg_s : Strategy_legal_snd g.init_game_state g.snd_legal fst_s (zGame_World.fst_strat_conditioned g f_strat))
+  (Leg_f : Strategy_legal_fst g.init_game_state g.fst_legal fst_s (zGame_World_wDraw.fst_strat_conditioned g f_strat))
+  (Leg_s : Strategy_legal_snd g.init_game_state g.snd_legal fst_s (zGame_World_wDraw.fst_strat_conditioned g f_strat))
+  (wlg_d : ¬Game_World_wDraw.draw_states g.toGame_World_wDraw g.init_game_state)
   (wlg_ws : ¬Game_World.snd_win_states g.toGame_World g.init_game_state)
   (hw : let f_act := fst_s g.init_game_state []
-        Game.fst_win { toGame_World := (g.world_after_fst f_act f_act_leg).toGame_World,
+        Game_wDraw.fst_win { toGame_World_wDraw := (g.world_after_fst f_act f_act_leg).toGame_World_wDraw,
                               fst_strat := f_strat [f_act] (by apply List.cons_ne_nil) f_act_leg,
                               snd_strat := g.snd_strat_conditioned fst_s f_act,
                               fst_lawful :=
                                 (by
                                 have := g.conditioned_legal_snd fst_s f_strat h_f_strat f_act_leg
                                 dsimp at this
-                                rw [zGame_World.world_after_fst_fst_legal, ← this]
+                                rw [zGame_World_wDraw.world_after_fst_fst_legal, ← this]
                                 exact Leg_s),
                               snd_lawful :=
                                 (by
                                 have := g.conditioned_legal_fst fst_s f_strat h_f_strat f_act_leg
                                 dsimp at this
-                                rw [zGame_World.world_after_fst_snd_legal, ← this]
+                                rw [zGame_World_wDraw.world_after_fst_snd_legal, ← this]
                                 exact Leg_f),
                                 }) :
-    Game.snd_win { toGame_World := g.toGame_World,
+    Game_wDraw.snd_win { toGame_World_wDraw := g.toGame_World_wDraw,
                           fst_strat := fst_s,
-                          snd_strat := (zGame_World.fst_strat_conditioned g f_strat),
+                          snd_strat := (zGame_World_wDraw.fst_strat_conditioned g f_strat),
                           fst_lawful := (Leg_f),
                           snd_lawful := (Leg_s)} :=
   by
@@ -1297,61 +1418,15 @@ lemma Conditioning_win [Inhabited β] (g : zGame_World α β) (fst_s: Strategy �
       apply g.state_on_turn_conditioned fst_s f_strat h_f_strat f_act_leg
     · intro n nt
       cases' n with n
-      · dsimp [Game.state_on_turn_neutral]
+      · dsimp [Game_wDraw.state_on_turn_neutral]
         rw [if_neg (by decide)]
-        dsimp [Game.state_on_turn]
-        exact wlg_ws
+        dsimp [Game_wDraw.state_on_turn]
+        constructor
+        · exact wlg_d
+        · exact wlg_ws
       · have := g.conditioned_state_on_turn_neutral fst_s f_strat h_f_strat f_act_leg n
-        apply Game.state_on_turn_neutral_from_World _ (n+1)
+        apply Game_wDraw.state_on_turn_neutral_from_World _ (n+1)
         dsimp
         rw [this]
         apply tn
         exact Nat.lt_of_add_lt_add_right nt
-
-
--- # Even more conditioining
-
-def zGame_World.snd_strat_deconditioned (s_strat : Strategy α β) (f_act : β) (g : zGame_World α β) (f_act_leg : g.fst_legal g.init_game_state [] f_act) : Strategy α β :=
-  fun _ hist => if hist = [] then f_act else s_strat (g.world_after_fst f_act f_act_leg).init_game_state (hist.dropLast)
-
-
-
-#exit
-
--- hmmmmm
-lemma Game_World.History_of_preconditioned
-  (g: Game_World α β)
-  (fst_act: β)
-  (f_strat s_strat : Strategy α β)
-  (turn : ℕ):
-  let fst_strat : Strategy α β := (fun _ hist => if hist = [] then fst_act else s_strat (g.world_after_fst fst_act).init_game_state (hist.dropLast)) ;
-  let snd_strat : Strategy α β := (fun _ hist => f_strat (g.world_after_fst fst_act).init_game_state (hist.dropLast)) ;
-  History_on_turn g.init_game_state fst_strat snd_strat (turn + 1) =
-  (History_on_turn (g.world_after_fst fst_act).init_game_state f_strat s_strat turn) ++ [fst_act] :=
-  by
-  intro fst_strat snd_strat
-  induction' turn with t ih
-  · dsimp [History_on_turn, Turn_fst]
-    rw [if_pos (by decide), if_pos (by rfl)]
-  · dsimp only [History_on_turn] at *
-    by_cases q : Turn_fst (t+1)
-    · rw [Turn_fst_not_step] at q
-      rw [if_neg q] at *
-      rw [← Turn_fst_not_step] at q
-      rw [if_pos q, if_pos q] at *
-      rw [List.cons_append, ← ih]
-      congr
-      dsimp at ih
-      rw [← Game_World.world_after_fst_init] at ih
-      rw [ih]
-      rw [List.dropLast_concat]
-    · rw [if_neg q, if_neg q] at *
-      rw [Turn_fst_not_step, not_not] at q
-      rw [if_pos q] at *
-      rw [if_neg (by apply List.cons_ne_nil)]
-      rw [List.cons_append, ← ih]
-      congr
-      dsimp at ih
-      rw [← Game_World.world_after_fst_init] at ih
-      rw [ih]
-      rw [List.dropLast_concat]
