Games/gameLib/Termination.lean
@@ -7,11 +7,21 @@ Author: Yves Jäckle.
 import Games.gameLib.Basic
 
 
+inductive Game_World.Turn_isWL (g : Game_World α β) (f_strat s_strat : Strategy α β) (turn : ℕ) : Prop where
+| wf : Turn_fst turn → g.fst_win_states (g.state_on_turn f_strat s_strat turn) → g.Turn_isWL f_strat s_strat turn
+| ws : Turn_snd turn → g.snd_win_states (g.state_on_turn f_strat s_strat turn) → g.Turn_isWL f_strat s_strat turn
 
 inductive Game_World_wDraw.Turn_isWLD (g : Game_World_wDraw α β) (f_strat s_strat : Strategy α β) (turn : ℕ) : Prop where
 | wf : Turn_fst turn → g.fst_win_states (g.state_on_turn f_strat s_strat turn) → g.Turn_isWLD f_strat s_strat turn
 | ws : Turn_snd turn → g.snd_win_states (g.state_on_turn f_strat s_strat turn) → g.Turn_isWLD f_strat s_strat turn
 | d : g.draw_states (g.state_on_turn f_strat s_strat turn) → g.Turn_isWLD f_strat s_strat turn
+
+
+def Game_World.isWL (g : Game_World α β) : Prop :=
+    ∀ f_strat s_strat : Strategy α β,
+    (f_leg : Strategy_legal_fst g.init_game_state g.fst_legal f_strat s_strat) →
+    (s_leg : Strategy_legal_snd g.init_game_state g.snd_legal f_strat s_strat) →
+    ∃ turn, g.Turn_isWL f_strat s_strat turn
 
 
 def Game_World_wDraw.isWLD (g : Game_World_wDraw α β) : Prop :=
@@ -24,6 +34,12 @@ def Game_World_wDraw.isWLD (g : Game_World_wDraw α β) : Prop :=
 structure Game_World_Terminating (α β : Type u) extends Game_World_wDraw α β where
   termination : toGame_World_wDraw.isWLD
 
+
+def Game_World.isWL_wBound (g : Game_World α β) (T : ℕ) : Prop :=
+    ∀ f_strat s_strat : Strategy α β,
+    (f_leg : Strategy_legal_fst g.init_game_state g.fst_legal f_strat s_strat) →
+    (s_leg : Strategy_legal_snd g.init_game_state g.snd_legal f_strat s_strat) →
+    ∃ turn ≤ T, g.Turn_isWL f_strat s_strat turn
 
 def Game_World_wDraw.isWLD_wBound (g : Game_World_wDraw α β) (T : ℕ) : Prop :=
     ∀ f_strat s_strat : Strategy α β,
@@ -113,7 +129,12 @@ lemma Game_wDraw.state_on_turn_neutral_from_World {α β : Type u} (g : Game_wDr
   intro w
   convert w
 
-
+lemma Game.state_on_turn_neutral_from_World {α β : Type u} (g : Game α β) (turn : ℕ) :
+  g.toGame_World.state_on_turn_neutral g.fst_strat g.snd_strat t → g.state_on_turn_neutral t :=
+  by
+  dsimp [Game_World.state_on_turn_neutral]
+  intro w
+  convert w
 
 @[simp]
 lemma Symm_Game.state_on_turn_neutral_toWorld {α β : Type u} (g : Symm_Game α β) :
