Games/gameLib/Zermelo.lean
@@ -13,40 +13,32 @@ import Mathlib.Tactic
 
 
 
-inductive zGame_World_wDraw.State_is_ws_d (g : zGame_World_wDraw α β) (s : α) : Prop where
-| ws : g.snd_win_states s → g.State_is_ws_d s
-| d : g.draw_states s → g.State_is_ws_d s
-
-lemma zGame_World_wDraw.init_wld_of_turn_zero_wld
-  (g : zGame_World_wDraw α β)
+lemma zGame_World.init_WL_of_turn_zero_WL
+  (g : zGame_World α β)
   (f_strat s_strat : Strategy α β):
-  g.Turn_isWLD f_strat s_strat 0 → g.State_is_ws_d g.init_game_state :=
+  g.Turn_isWL f_strat s_strat 0 → g.snd_win_states g.init_game_state :=
   by
   intro t0
-  cases' t0 with wf ws d
+  cases' t0 with wf ws
   · contradiction
   · rename_i h
-    dsimp [Game_World_wDraw.state_on_turn] at h
-    apply zGame_World_wDraw.State_is_ws_d.ws
-    exact h
-  · rename_i h
-    dsimp [Game_World_wDraw.state_on_turn] at h
-    apply zGame_World_wDraw.State_is_ws_d.d
+    dsimp [Game_World.state_on_turn] at h
     exact h
 
 
-lemma zGame_World_wDraw.conditioning_bound
-  (g : zGame_World_wDraw α β)
-  {T : ℕ} (hg : g.isWLD_wBound (T + 1))
+
+lemma zGame_World.conditioning_bound
+  (g : zGame_World α β)
+  {T : ℕ} (hg : g.isWL_wBound (T + 1))
   (fst_act : β) (leg : g.fst_legal g.init_game_state [] fst_act) :
-  (g.toGame_World_wDraw.world_after_fst fst_act).isWLD_wBound T :=
+  (g.toGame_World.world_after_fst fst_act).isWL_wBound T :=
   by
   have nt := g.coherent
-  have b := Game_World_wDraw.strong_legal_blind_toWeak _ (Game_World_wDraw.hyper_legal_blind_toStrong _ g.is_hyper_legal_blind)
-  have tb := Game_World_wDraw.strong_transition_blind_toWeak _ (Game_World_wDraw.hyper_transition_blind_toStrong _ g.is_hyper_transition_blind)
+  have b := Game_World.strong_legal_blind_toWeak _ (Game_World.hyper_legal_blind_toStrong _ g.is_hyper_legal_blind)
+  have tb := Game_World.strong_transition_blind_toWeak _ (Game_World.hyper_transition_blind_toStrong _ g.is_hyper_transition_blind)
   intro f_strat s_strat f_leg s_leg
-  let fst_strat : Strategy α β := fst_strat_deconditioned s_strat fst_act g.toGame_World_wDraw
-  let snd_strat : Strategy α β := snd_strat_deconditioned f_strat fst_act g.toGame_World_wDraw
+  let fst_strat : Strategy α β := fst_strat_deconditioned s_strat fst_act g.toGame_World
+  let snd_strat : Strategy α β := snd_strat_deconditioned f_strat fst_act g.toGame_World
   specialize hg fst_strat snd_strat _ _
   · apply g.fst_legal_deconditioned fst_act leg  f_strat s_strat s_leg b.1
   · apply g.snd_legal_deconditioned fst_act leg  f_strat s_strat f_leg b.2
@@ -58,976 +50,184 @@ lemma zGame_World_wDraw.conditioning_bound
       · cases' t_prop
         · rename_i no pe ; contradiction
         · rename_i c
-          apply Game_World_wDraw.Turn_isWLD.ws
+          apply Game_World.Turn_isWL.ws
           · decide
-          · dsimp [Game_World_wDraw.state_on_turn]
+          · dsimp [Game_World.state_on_turn]
             have := (nt fst_strat snd_strat 0).s c
-            dsimp [Game_World_wDraw.state_on_turn] at this
+            dsimp [Game_World.state_on_turn] at this
             rw [if_pos (by decide)] at this
-            dsimp [Game_World_wDraw.history_on_turn, History_on_turn, fst_strat_deconditioned] at this
+            dsimp [Game_World.history_on_turn, History_on_turn, fst_strat_deconditioned] at this
             rw [if_pos (by rfl)] at this
             exact this
-        · rename_i c
-          apply Game_World_wDraw.Turn_isWLD.d
-          dsimp [Game_World_wDraw.state_on_turn]
-          have := (nt fst_strat snd_strat 0).d c
-          dsimp [Game_World_wDraw.state_on_turn] at this
-          rw [if_pos (by decide)] at this
-          dsimp [Game_World_wDraw.history_on_turn, History_on_turn, fst_strat_deconditioned] at this
-          rw [if_pos (by rfl)] at this
-          exact this
     · rw [Nat.succ_le_succ_iff] at t_bd
       use t
       constructor
       · exact t_bd
       · cases' t_prop with tp c tp c c
-        · apply Game_World_wDraw.Turn_isWLD.ws
+        · apply Game_World.Turn_isWL.ws
           · rw [Turn_snd_fst_step] ; exact tp
-          · rw [← Game_World_wDraw.State_of_deconditioned]
-            · rw [Game_World_wDraw.world_after_fst_snd_win_states]
+          · rw [← Game_World.State_of_deconditioned]
+            · rw [Game_World.world_after_fst_snd_win_states]
               rw [g.sym_win] at c
               exact c
             · exact tb
             · exact leg
-        · apply Game_World_wDraw.Turn_isWLD.wf
+        · apply Game_World.Turn_isWL.wf
           · rw [Turn_fst_snd_step] ; exact tp
-          · rw [← Game_World_wDraw.State_of_deconditioned]
-            · rw [Game_World_wDraw.world_after_fst_fst_win_states]
+          · rw [← Game_World.State_of_deconditioned]
+            · rw [Game_World.world_after_fst_fst_win_states]
               rw [← g.sym_win] at c
               exact c
             · exact tb
             · exact leg
-        · apply Game_World_wDraw.Turn_isWLD.d
-          · rw [← Game_World_wDraw.State_of_deconditioned]
-            · rw [Game_World_wDraw.world_after_fst_draw_states]
-              exact c
-            · exact tb
-            · exact leg
 
 
 
-lemma zGame_World_wDraw.conditioning_WLD_helper
-  (g : zGame_World_wDraw α β)
-  (hwld : g.has_WLD)
-  (hnfw : ¬ g.is_snd_win)
-  (hnd : ¬ g.is_draw) :
+
+lemma zGame_World.conditioning_WL_helper
+  (g : zGame_World α β)
+  (hWL : g.has_WL)
+  (hnfw : ¬ g.is_snd_win) :
   g.is_fst_win :=
   by
-  cases' hwld
+  cases' hWL
   · assumption
   · contradiction
-  · contradiction
 
 
 
 
-lemma zGame_World_wDraw.conditioning_WLD
+lemma zGame_World.conditioning_WL
   [Inhabited β]
-  (g : zGame_World_wDraw α β)
-  (h : ∀ fst_act : β, (hl : g.fst_legal g.init_game_state [] fst_act) → (g.world_after_fst fst_act hl).has_WLD)
+  (g : zGame_World α β)
+  (h : ∀ fst_act : β, (hl : g.fst_legal g.init_game_state [] fst_act) → (g.world_after_fst fst_act hl).has_WL)
   :
-  g.has_WLD :=
+  g.has_WL :=
   by
   classical
-  apply g.has_WLD_init_end _ h
-  rintro ⟨_,wlg_d,wlg_ws⟩
+  apply g.has_WL_init_end _ h
+  rintro ⟨_,wlg⟩
   by_cases qws : ∃ f_act : β, ∃ (hl : g.fst_legal g.init_game_state [] f_act), (g.world_after_fst f_act hl).is_snd_win
   · obtain ⟨f_act, f_act_leg, ws, ws_prop⟩ := qws
-    apply zGame_World_wDraw.has_WLD.wf
-    sorry
-  · push_neg at qws
-    by_cases qd : ∃ f_act : β, ∃ (hl : g.fst_legal g.init_game_state [] f_act), (g.world_after_fst f_act hl).is_draw
-    · obtain ⟨f_act, f_act_leg, d⟩ := qd
-      apply zGame_World_wDraw.has_WLD.d
-      sorry
-    · sorry
-      -- push_neg at qd
-      -- apply zGame_World_wDraw.has_WLD.ws
-      -- let ws_aux (hi : List β) (hne : hi ≠ [])  (hil : g.fst_legal g.init_game_state [] (hi.getLast hne)) :=
-      --   let f_act := List.getLast hi hne
-      --   (Classical.choose ((g.world_after_fst f_act hil).conditioning_WLD_helper
-      --                                                         (h f_act hil)
-      --                                                         (qws f_act hil)
-      --                                                         (qd f_act hil)))
-      -- let ws : Strategy α β := fun (ini : α) hist  =>
-      --                           if hh : hist = [] -- shouldn't happen, as snd strat
-      --                           then default -- dummy
-      --                           else let f_act := List.getLast hist hh
-      --                                if H : g.fst_legal g.init_game_state [] f_act-- should be the cases ?!?
-      --                                then (ws_aux hist hh H)
-      --                                      (g.fst_transition g.init_game_state [] f_act) hist.dropLast -- is it ? since ref to history in current game
-      --                                else default
-      -- use ws
-      -- intro f_strat ws_leg f_leg
-      -- let f_act := f_strat g.init_game_state []
-      -- have f_act_leg := f_leg 0 (by decide)
-      -- dsimp [History_on_turn] at f_act_leg
+    apply zGame_World.has_WL.wf
+    use (g.snd_strat_deconditioned ws f_act f_act_leg)
+    intro snd_s ws_leg snd_leg
 
-      -- have fix : ∀ (h H : List β) (hne : h ≠ []) (Hne : H ≠ [])
-      --           (hl : Game_World.fst_legal g.toGame_World g.init_game_state [] (List.getLast h hne))
-      --           (Hl : Game_World.fst_legal g.toGame_World g.init_game_state [] (List.getLast H Hne)),
-      --           List.getLast h hne = List.getLast H Hne → ws_aux h hne hl = ws_aux H Hne Hl :=
-      --   by
-      --   intro h H hne Hne hl Hl main
-      --   dsimp [ws_aux]
-      --   simp_rw [main]
+  · sorry
+    -- push_neg at qws
+    -- apply zGame_World.has_WL.ws
+    -- let ws_aux (hi : List β) (hne : hi ≠ [])  (hil : g.fst_legal g.init_game_state [] (hi.getLast hne)) :=
+    --   let f_act := List.getLast hi hne
+    --   (Classical.choose ((g.world_after_fst f_act hil).conditioning_WL_helper
+    --                                                         (h f_act hil)
+    --                                                         (qws f_act hil)
+    --                                                         --(qd f_act hil))
+    --                                                         ))
+    -- let ws : Strategy α β := fun (ini : α) hist  =>
+    --                           if hh : hist = [] -- shouldn't happen, as snd strat
+    --                           then default -- dummy
+    --                           else let f_act := List.getLast hist hh
+    --                                 if H : g.fst_legal g.init_game_state [] f_act-- should be the cases ?!?
+    --                                 then (ws_aux hist hh H)
+    --                                       (g.fst_transition g.init_game_state [] f_act) hist.dropLast -- is it ? since ref to history in current game
+    --                                 else default
+    -- use ws
+    -- intro f_strat ws_leg f_leg
+    -- let f_act := f_strat g.init_game_state []
+    -- have f_act_leg := f_leg 0 (by decide)
+    -- dsimp [History_on_turn] at f_act_leg
 
-      -- have proof := ((g.world_after_fst f_act f_act_leg).conditioning_WLD_helper
-      --                                 (h f_act f_act_leg)
-      --                                 (qws f_act f_act_leg)
-      --                                 (qd f_act f_act_leg))
-      -- have da_prop := Classical.choose_spec proof
-      -- specialize da_prop (g.snd_strat_conditioned f_strat f_act)
-      -- specialize da_prop (by
-      --                     have := g.conditioned_legal_snd f_strat ws_aux fix f_act_leg
-      --                     dsimp [ws_aux] at this
-      --                     simp_rw [zGame_World_wDraw.world_after_fst_fst_legal]
-      --                     rw [← this]
-      --                     apply Strategy_legal_snd_eq_strats_snd g f_strat ws (g.fst_strat_conditioned ws_aux)
-      --                     · intro t ts
-      --                       cases' t with t
-      --                       · contradiction
-      --                       · dsimp [ws, fst_strat_conditioned]
-      --                         rw [dif_neg (by apply History_on_turn_nonempty_of_succ)]
-      --                         rw [History_on_turn_getLast_fst_act]
-      --                         rw [dif_pos f_act_leg]
-      --                         rw [dif_neg (by apply History_on_turn_nonempty_of_succ)]
-      --                         rw [History_on_turn_getLast_fst_act]
-      --                         rw [dif_pos f_act_leg]
-      --                         rfl
-      --                     · exact ws_leg
-      --                     )
-      -- specialize da_prop (by
-      --                     have := g.conditioned_legal_fst f_strat ws_aux fix f_act_leg
-      --                     dsimp [ws_aux] at this
-      --                     simp_rw [zGame_World_wDraw.world_after_fst_snd_legal]
-      --                     rw [← this]
-      --                     apply Strategy_legal_fst_eq_strats_snd g f_strat ws (g.fst_strat_conditioned ws_aux)
-      --                     · intro t ts
-      --                       cases' t with t
-      --                       · contradiction
-      --                       · dsimp [ws, fst_strat_conditioned]
-      --                         rw [dif_neg (by apply History_on_turn_nonempty_of_succ)]
-      --                         rw [History_on_turn_getLast_fst_act]
-      --                         rw [dif_pos f_act_leg]
-      --                         rw [dif_neg (by apply History_on_turn_nonempty_of_succ)]
-      --                         rw [History_on_turn_getLast_fst_act]
-      --                         rw [dif_pos f_act_leg]
-      --                         rfl
-      --                     · exact f_leg
-      --                     )
-      -- apply Conditioning_win
-      -- · exact wlg_d
-      -- · exact wlg_ws
-      -- · apply da_prop
-      -- · exact fix
+    -- have fix : ∀ (h H : List β) (hne : h ≠ []) (Hne : H ≠ [])
+    --           (hl : Game_World.fst_legal g.toGame_World g.init_game_state [] (List.getLast h hne))
+    --           (Hl : Game_World.fst_legal g.toGame_World g.init_game_state [] (List.getLast H Hne)),
+    --           List.getLast h hne = List.getLast H Hne → ws_aux h hne hl = ws_aux H Hne Hl :=
+    --   by
+    --   intro h H hne Hne hl Hl main
+    --   dsimp [ws_aux]
+    --   simp_rw [main]
+
+    -- have proof := ((g.world_after_fst f_act f_act_leg).conditioning_WL_helper
+    --                                 (h f_act f_act_leg)
+    --                                 (qws f_act f_act_leg)
+    --                                 --(qd f_act f_act_leg)
+    --                                 )
+    -- have da_prop := Classical.choose_spec proof
+    -- specialize da_prop (g.snd_strat_conditioned f_strat f_act)
+    -- specialize da_prop (by
+    --                     have := g.conditioned_legal_snd f_strat ws_aux fix f_act_leg
+    --                     dsimp [ws_aux] at this
+    --                     simp_rw [zGame_World.world_after_fst_fst_legal]
+    --                     rw [← this]
+    --                     apply Strategy_legal_snd_eq_strats_snd g f_strat ws (g.fst_strat_conditioned ws_aux)
+    --                     · intro t ts
+    --                       cases' t with t
+    --                       · contradiction
+    --                       · dsimp [ws, fst_strat_conditioned]
+    --                         rw [dif_neg (by apply History_on_turn_nonempty_of_succ)]
+    --                         rw [History_on_turn_getLast_fst_act]
+    --                         rw [dif_pos f_act_leg]
+    --                         rw [dif_neg (by apply History_on_turn_nonempty_of_succ)]
+    --                         rw [History_on_turn_getLast_fst_act]
+    --                         rw [dif_pos f_act_leg]
+    --                         rfl
+    --                     · exact ws_leg
+    --                     )
+    -- specialize da_prop (by
+    --                     have := g.conditioned_legal_fst f_strat ws_aux fix f_act_leg
+    --                     dsimp [ws_aux] at this
+    --                     simp_rw [zGame_World.world_after_fst_snd_legal]
+    --                     rw [← this]
+    --                     apply Strategy_legal_fst_eq_strats_snd g f_strat ws (g.fst_strat_conditioned ws_aux)
+    --                     · intro t ts
+    --                       cases' t with t
+    --                       · contradiction
+    --                       · dsimp [ws, fst_strat_conditioned]
+    --                         rw [dif_neg (by apply History_on_turn_nonempty_of_succ)]
+    --                         rw [History_on_turn_getLast_fst_act]
+    --                         rw [dif_pos f_act_leg]
+    --                         rw [dif_neg (by apply History_on_turn_nonempty_of_succ)]
+    --                         rw [History_on_turn_getLast_fst_act]
+    --                         rw [dif_pos f_act_leg]
+    --                         rfl
+    --                     · exact f_leg
+    --                     )
+    -- apply Conditioning_win
+    -- · exact wlg
+    -- · apply da_prop
+    -- · exact fix
 
 
 
 
---#exit
 
-lemma zGame_World_wDraw.Zermelo
+
+lemma zGame_World.Zermelo
   [Inhabited β]
-  (g : zGame_World_wDraw α β)
-  {T : ℕ} (hg : g.isWLD_wBound T)
-  : g.has_WLD :=
+  (g : zGame_World α β)
+  {T : ℕ} (hg : g.isWL_wBound T)
+  : g.has_WL :=
   by
   revert g
   induction' T with t ih
   · intro g t0
-    dsimp [Game_World_wDraw.isWLD_wBound] at t0
+    dsimp [Game_World.isWL_wBound] at t0
     obtain ⟨f_strat, s_strat, f_leg, s_leg⟩ := g.playable_has_strat g.playable
     obtain ⟨t, tl0, t_end⟩ := t0 f_strat s_strat f_leg s_leg
     rw [Nat.le_zero] at tl0
     rw [tl0] at t_end
-    replace t_end := g.init_wld_of_turn_zero_wld f_strat s_strat t_end
-    cases' t_end
-    · apply zGame_World_wDraw.has_WLD.ws
-      use (fun _ _ => default)
-      intro f_strat' leg f_leg'
-      use 0
-      constructor
-      · decide
-      · constructor
-        · dsimp [Game.state_on_turn]
-          rename_i h ; exact h
-        · intro t ahhh ; contradiction
-    · apply zGame_World_wDraw.has_WLD.d
-      right
-      use (fun _ _ => default)
-      intro f_strat' leg f_leg'
-      use 0
-      constructor
-      · decide
-      · constructor
-        · dsimp [Game.state_on_turn]
-          rename_i h ; exact h
-        · intro t ahhh ; contradiction
+    replace t_end := g.init_WL_of_turn_zero_WL f_strat s_strat t_end
+    apply zGame_World.has_WL.ws
+    use (fun _ _ => default)
+    intro f_strat' leg f_leg'
+    use 0
+    constructor
+    · decide
+    · constructor
+      · dsimp [Game.state_on_turn]
+        exact t_end
+      · intro t ahhh ; contradiction
   · intro g bd
-    apply zGame_World_wDraw.conditioning_WLD
+    apply zGame_World.conditioning_WL
     intro f_act f_leg
     apply ih
-    exact zGame_World_wDraw.conditioning_bound g bd f_act f_leg
-
-
-
-#exit
-
-
--- # Initial stuff
-
-inductive Game.is_win_loose_draw {α β : Type u} (g : Game α β) : Prop
-| win_f : g.fst_win → g.is_win_loose_draw
-| win_s : g.snd_win → g.is_win_loose_draw
-| draw : g.draw → g.is_win_loose_draw
-
-
-lemma Game.terminates_is_win_loose_draw {α β : Type u} (g : Game α β)
-  (hg : g.terminates) : g.is_win_loose_draw :=
-  by
-  rw [Game.terminates] at hg
-  obtain ⟨end_turn, end_turn_prop⟩ := hg
-  by_cases q : (∀ t ≤ end_turn, g.state_on_turn_neutral t)
-  · apply Game.is_win_loose_draw.draw
-    use end_turn
-  · push_neg at q
-    have wf : _ := Nat.lt_wfRel.wf
-    rw [WellFounded.wellFounded_iff_has_min] at wf
-    specialize wf (fun t => t ≤ end_turn → ¬state_on_turn_neutral g t)
-    dsimp [Set.Nonempty, Membership.mem, Set.Mem] at wf
-    obtain ⟨it, it_bound, it_prop⟩ := q
-    specialize wf ⟨it, (show _ from by intro ; exact it_prop)⟩
-    obtain ⟨nnt, nnt_prop, nnt_min⟩ := wf
-    have fact : nnt ≤ end_turn :=
-      by
-      apply le_trans _ it_bound
-      specialize nnt_min it (show _ from by intro ; exact it_prop)
-      rw [WellFoundedRelation.rel] at nnt_min
-      rw [Game.state_on_turn_neutral] at nnt_prop
-      -- I don't know why there's trouble here
-      by_contra con
-      rw [not_le] at con
-      exact nnt_min con
-    specialize nnt_prop fact
-    rw [Game.state_on_turn_neutral] at nnt_prop
-    split_ifs at nnt_prop with tc
-    · rw [not_not] at nnt_prop
-      apply Game.is_win_loose_draw.win_f
-      use nnt
-      constructor
-      · exact tc
-      · constructor
-        · exact nnt_prop
-        · intro t t_lt
-          by_contra k
-          specialize nnt_min t (show _ from by intro ; exact k)
-          exact nnt_min t_lt
-    · rw [not_not] at nnt_prop
-      apply Game.is_win_loose_draw.win_s
-      use nnt
-      constructor
-      · exact tc
-      · constructor
-        · exact nnt_prop
-        · intro t t_lt
-          by_contra k
-          specialize nnt_min t (show _ from by intro ; exact k)
-          exact nnt_min t_lt
-
-inductive Symm_Game.is_win_loose_draw {α β : Type u} (g : Symm_Game α β) : Prop
-| win_f : g.fst_win → g.is_win_loose_draw
-| win_s : g.snd_win → g.is_win_loose_draw
-| draw : g.draw → g.is_win_loose_draw
-
-@[simp]
-lemma Symm_Game.is_win_loose_draw_toGame {α β : Type u} (g : Symm_Game α β) :
-  g.toGame.is_win_loose_draw ↔ g.is_win_loose_draw :=
-  by
-  constructor
-  · intro G
-    cases G with
-    | win_f f => apply Symm_Game.is_win_loose_draw.win_f ; exact f
-    | win_s s => apply Symm_Game.is_win_loose_draw.win_s ; exact s
-    | draw f => apply Symm_Game.is_win_loose_draw.draw ; exact f
-  · intro G
-    cases G with
-    | win_f f => apply Game.is_win_loose_draw.win_f ; exact f
-    | win_s s => apply Game.is_win_loose_draw.win_s ; exact s
-    | draw f => apply Game.is_win_loose_draw.draw ; exact f
-
-
-lemma Symm_Game.terminates_is_win_loose_draw {α β : Type u} (g : Symm_Game α β)
-  (hg : g.terminates) : g.is_win_loose_draw :=
-  by
-  rw [← Symm_Game.terminates_toGame] at hg
-  rw [← Symm_Game.is_win_loose_draw_toGame]
-  exact Game.terminates_is_win_loose_draw (toGame g) hg
-
-
-inductive Game_World.has_win_loose_draw_strat {α β : Type u} (g : Game_World α β) : Prop
-| win_f : g.is_fst_win → g.has_win_loose_draw_strat
-| win_s : g.is_snd_win → g.has_win_loose_draw_strat
-| draw : g.is_draw → g.has_win_loose_draw_strat
-
-
-def Game_World.playable_fst {α β : Type u} (g : Game_World α β) : Prop :=
-  (∃ e : Strategy α β, ∀ s : Strategy α β, Strategy_legal g.init_game_state (fun _ => g.fst_legal) e s e)
-
-def Game_World.playable_snd {α β : Type u} (g : Game_World α β) : Prop :=
-  (∃ e : Strategy α β, ∀ s : Strategy α β, Strategy_legal g.init_game_state (fun _ => g.snd_legal) s e e)
-
-def Game_World.playable {α β : Type u} (g : Game_World α β) : Prop :=
-  g.playable_fst ∧ g.playable_snd
-
--- non-playable worlds are for example those with law `fun _ _ _ => False`
-
-
-def Game_World.playable' {α β : Type u} (g : Game_World α β) : Prop :=
-  ∃ f : Strategy α β, ∃ s : Strategy α β,
-    (Strategy_legal g.init_game_state (fun _ => g.fst_legal) f s f)
-    ∧ (Strategy_legal g.init_game_state (fun _ => g.snd_legal) f s s)
-
-
-
-def Game_World.world_after_fst {α β : Type u} (g : Game_World α β)
-  (fst_act : β) : Game_World α β := -- act not required to be legal
-  {g with init_game_state := g.fst_transition [] fst_act }
-  -- maybe swap fst and snd notions ? Cause we expect snd player to go fst now
-
-@[simp]
-lemma Game_World.world_after_fst_init {α β : Type u} (g : Game_World α β)
-  (fst_act : β) : (g.world_after_fst fst_act).init_game_state = g.fst_transition [] fst_act :=
-  by rfl
-
-@[simp]
-lemma Game_World.world_after_fst_fst_trans {α β : Type u} (g : Game_World α β)
-  (fst_act : β) : (g.world_after_fst fst_act).fst_transition = g.fst_transition :=
-  by rfl
-
-@[simp]
-lemma Game_World.world_after_fst_snd_trans {α β : Type u} (g : Game_World α β)
-  (fst_act : β) : (g.world_after_fst fst_act).snd_transition = g.snd_transition :=
-  by rfl
-
-@[simp]
-lemma Game_World.world_after_fst_fst_legal {α β : Type u} (g : Game_World α β)
-  (fst_act : β) : (g.world_after_fst fst_act).fst_legal = g.fst_legal :=
-  by rfl
-
-@[simp]
-lemma Game_World.world_after_fst_snd_legal {α β : Type u} (g : Game_World α β)
-  (fst_act : β) : (g.world_after_fst fst_act).snd_legal = g.snd_legal :=
-  by rfl
-
-
-/-
-In chess, imaging a board with pieces at random, and consider two situations.
-In the first, the first player makes a move and then the second one does.
-In the second situation, the board is that of the first situation, but we ask the
-second player to move first. Will the second players moves be the same in both
-situations ?
-They don't have to. After all, in the first scenario, the second player gains
-some knowledge about how the first plays...
-We'll call strategies that play the same in both situations "careless".
--/
-
-def Game_World.Strategy_careless (strat : Strategy α β) (g : Game_World α β): Prop :=
-  ∀ f_act : β, ∀ hist : List β, strat (g.fst_transition [] f_act) hist = strat g.init_game_state (hist ++ [f_act])
-
-/-
-In ↑, we can't just have hist = [] and deduce the ↑ from this case : the moves
-for these two scenarios may be the same at that stage, but they could begin
-to differ at future stages
-
-Example for PUB in `Careless_Example`
--/
-
-def Symm_Game_World.Strategy_careless (strat : Strategy α β) (g : Symm_Game_World α β): Prop :=
-  ∀ f_act : β, ∀ hist : List β, strat (g.transition [] f_act) hist = strat g.init_game_state (hist ++ [f_act])
-
-
-
-lemma Game_World.world_after_fst_History (g : Game_World α β)
-  (f_strat s_strat : Strategy α β) (turn : ℕ)
-  (hs : g.Strategy_careless s_strat) (hf : g.Strategy_careless f_strat) :
-  (History_on_turn (g.world_after_fst (f_strat g.init_game_state [])).init_game_state s_strat f_strat turn)
-  ++ [(f_strat g.init_game_state [])] = History_on_turn g.init_game_state f_strat s_strat (turn+1) :=
-  by
-  rw [History_on_turn]
-  induction' turn with t ih
-  · dsimp [History_on_turn]
-    rw [if_pos (by decide)]
-  · dsimp [History_on_turn]
-    by_cases q : Turn_fst (t+1)
-    · rw [if_pos q] at *
-      rw [Turn_fst_not_step] at q
-      rw [if_neg q]
-      rw [← Turn_fst_not_step] at q
-      rw [if_pos q]
-      rw [Game_World.world_after_fst_init] at *
-      rw [List.cons_append, ih]
-      congr 1
-      rw [hs, ih]
-    · rw [if_neg q] at *
-      rw [Turn_fst_not_step, not_not] at q
-      rw [if_pos q]
-      rw [← @not_not (Turn_fst (t + 1 + 1)), ← Turn_fst_not_step] at q
-      rw [if_neg q]
-      rw [Game_World.world_after_fst_init] at *
-      rw [List.cons_append, ih]
-      congr 1
-      rw [hf, ih]
-
-
-
-lemma Game_World.Strategy_careless_act_on_turn_snd (g : Game_World α β) (f_strat s_strat: Strategy α β)
-  (hs : g.Strategy_careless s_strat) (hf : g.Strategy_careless f_strat) (turn : ℕ) :
-  s_strat (g.world_after_fst (f_strat g.init_game_state [])).init_game_state
-    (History_on_turn (g.world_after_fst (f_strat g.init_game_state [])).init_game_state s_strat f_strat turn) =
-  s_strat g.init_game_state (History_on_turn g.init_game_state f_strat s_strat (turn + 1)) :=
-  by
-  rw [Game_World.world_after_fst_init, hs]
-  congr
-  apply Game_World.world_after_fst_History g f_strat s_strat turn hs hf
-
-
-
-lemma Game_World.Strategy_careless_act_on_turn_fst (g : Game_World α β) (f_strat s_strat: Strategy α β)
-  (hs : g.Strategy_careless s_strat) (hf : g.Strategy_careless f_strat) (turn : ℕ) :
-  f_strat (g.world_after_fst (f_strat g.init_game_state [])).init_game_state
-    (History_on_turn (g.world_after_fst (f_strat g.init_game_state [])).init_game_state s_strat f_strat turn) =
-  f_strat g.init_game_state (History_on_turn g.init_game_state f_strat s_strat (turn + 1)) :=
-  by
-  rw [Game_World.world_after_fst_init, hf]
-  congr
-  apply Game_World.world_after_fst_History g f_strat s_strat turn hs hf
-
-/--
-The action is legal on turn t in the game with initial state being the state after f's first move,
-where s plays first and f second, iff it it legal on turn t+1 of the original game.
--/
-def Game_World.law_blind_fst (g : Game_World α β) (f_strat s_strat: Strategy α β) : Prop :=
-  ∀ turn : ℕ, ∀ act : β, g.snd_legal (History_on_turn (g.world_after_fst (f_strat g.init_game_state [])).init_game_state s_strat f_strat turn) act
-    ↔ g.fst_legal (History_on_turn g.init_game_state f_strat s_strat (turn + 1)) act
-
-def Game_World.law_blind_snd (g : Game_World α β) (f_strat s_strat: Strategy α β) : Prop :=
-  ∀ turn : ℕ, ∀ act : β, g.fst_legal (History_on_turn (g.world_after_fst (f_strat g.init_game_state [])).init_game_state s_strat f_strat turn) act
-    ↔ g.snd_legal (History_on_turn g.init_game_state f_strat s_strat (turn + 1)) act
-
-def Game_World.law_blind (g : Game_World α β) (f_strat s_strat: Strategy α β) : Prop :=
-  g.law_blind_fst f_strat s_strat ∧ g.law_blind_snd f_strat s_strat
-
-
-lemma Game_World.world_after_fst_legal (g : Game_World α β)
-   (f_strat s_strat: Strategy α β) (h : Strategy_legal g.init_game_state (fun x => g.fst_legal) f_strat s_strat f_strat)
-   (hs : g.Strategy_careless s_strat) (hf : g.Strategy_careless f_strat)
-   (hg : g.law_blind f_strat s_strat):
-   Strategy_legal (g.world_after_fst (f_strat g.init_game_state [])).init_game_state (fun x => (g.world_after_fst (f_strat g.init_game_state [])).snd_legal) s_strat f_strat f_strat :=
-   by
-   dsimp [Strategy_legal] at *
-   intro t
-   have := g.Strategy_careless_act_on_turn_fst f_strat s_strat hs hf t
-   rw [Game_World.world_after_fst_init] at this
-   rw [this]
-   clear this
-   obtain ⟨bf, bs⟩ := hg
-   specialize h (t+1)
-   specialize bf t (f_strat g.init_game_state (History_on_turn g.init_game_state f_strat s_strat (t + 1)))
-   rw [← Game_World.world_after_fst_init, bf]
-   exact h
-
-
-lemma Game_World.world_after_snd_legal (g : Game_World α β)
-   (f_strat s_strat: Strategy α β) (h : Strategy_legal g.init_game_state (fun x => g.snd_legal) f_strat s_strat s_strat)
-   (hs : g.Strategy_careless s_strat) (hf : g.Strategy_careless f_strat)
-   (hg : g.law_blind f_strat s_strat):
-   Strategy_legal (g.world_after_fst (f_strat g.init_game_state [])).init_game_state (fun x => (g.world_after_fst (f_strat g.init_game_state [])).fst_legal) s_strat f_strat s_strat :=
-   by
-   dsimp [Strategy_legal] at *
-   intro t
-   have := g.Strategy_careless_act_on_turn_snd f_strat s_strat hs hf t
-   rw [Game_World.world_after_fst_init] at this
-   rw [this]
-   clear this
-   obtain ⟨bf, bs⟩ := hg
-   specialize h (t+1)
-   specialize bs t (s_strat g.init_game_state (History_on_turn g.init_game_state f_strat s_strat (t + 1)))
-   rw [← Game_World.world_after_fst_init, bs]
-   exact h
-
-
-lemma Game_World.world_after_fst_legal' (g : Game_World α β)
-  (f_strat s_strat: Strategy α β)
-  (h : Strategy_legal (g.world_after_fst (f_strat g.init_game_state [])).init_game_state (fun x => g.snd_legal) s_strat f_strat f_strat)
-  (hi : fst_legal g [] (f_strat g.init_game_state []))
-  -- ↑ may not necessarily be ommitted. `f_strat g.init_game_state []` may not be legal, although
-  -- `f_strat` is legal if we take the latters transition as initial turn ...
-  (hs : g.Strategy_careless s_strat) (hf : g.Strategy_careless f_strat)
-  (hg : g.law_blind f_strat s_strat) :
-  Strategy_legal g.init_game_state (fun x => g.fst_legal) f_strat s_strat f_strat :=
-  by
-  dsimp [Strategy_legal] at *
-  intro t
-  cases' t with t
-  · dsimp [History_on_turn]
-    exact hi
-  · rw [← (hg.1 t), Game_World.world_after_fst_init]
-    rw [← Game_World.world_after_fst_History _ _ _ _ hs hf]
-    specialize h t
-    rw [← hf]
-    apply h
-
-
-lemma Game_World.world_after_snd_legal' (g : Game_World α β)
-  (f_strat s_strat: Strategy α β)
-  (h : Strategy_legal (g.world_after_fst (f_strat g.init_game_state [])).init_game_state (fun x => g.fst_legal) s_strat f_strat s_strat)
-  (hi : snd_legal g [] (s_strat g.init_game_state []))
-  -- ↑ never takes efect in practice, as second player doesn't have first turn,
-  -- so this case has to be handled in the non-partial defintiion of the second strat...
-  (hs : g.Strategy_careless s_strat) (hf : g.Strategy_careless f_strat)
-  (hg : g.law_blind f_strat s_strat) :
-  Strategy_legal g.init_game_state (fun x => g.snd_legal) f_strat s_strat s_strat :=
-  by
-  dsimp [Strategy_legal] at *
-  intro t
-  cases' t with t
-  · dsimp [History_on_turn]
-    exact hi
-  · rw [← (hg.2 t), Game_World.world_after_fst_init]
-    rw [← Game_World.world_after_fst_History _ _ _ _ hs hf]
-    specialize h t
-    rw [← hs]
-    apply h
-
-
--- needed for `Game_World.world_after_fst_init_must_terminate`
-instance (l : List α): Decidable (l = []) :=
-  by
-  match l with
-  | [] => apply isTrue ; rfl
-  | x :: L => apply isFalse ; exact List.cons_ne_nil x L
-
-
--- lemma name_1 (g : Game_World α β)
---   (fst_act: β)
---   (fst_act_legal: g.fst_legal [] fst_act)
---   (s_strat : Strategy α β) (turn : ℕ)
---   (hs : g.Strategy_careless s_strat) :
---   let fst_strat : Strategy α β := (fun ini hist => if hist = [] then fst_act else s_strat (g.world_after_fst fst_act).init_game_state (hist.dropLast)) ;
---   fst_strat g.init_game_state (History_on_turn g.init_game_state fst_strat s_strat (turn+1)) =
---   s_strat (g.world_after_fst fst_act).init_game_state (History_on_turn (g.world_after_fst (fst_act)).init_game_state s_strat fst_strat turn) :=
---   by
---   intro fst_strat
---   dsimp
---   rw [if_neg _]
---   swap
---   · dsimp [History_on_turn]
---     split_ifs <;> decide
---   · rw [← Game_World.world_after_fst_History]
---     · rw [if_pos (by rfl)]
---       rw [List.dropLast_concat]
---       rfl
---     · exact hs
---     · intro a h
---       cases' h with x l
---       · dsimp
---         specialize hs fst_act []
---         dsimp at hs
---         sorry -- add as hypo ?
-
--- lemma name_2 (g : Game_World α β)
---   (fst_act: β)
---   (fst_act_legal: g.fst_legal [] fst_act)
---   (s_strat : Strategy α β)
---   (hs : g.Strategy_careless s_strat) :
---   let fst_strat : Strategy α β := (fun ini hist => if hist = [] then fst_act else s_strat (g.world_after_fst fst_act).init_game_state (hist.dropLast)) ;
---   g.Strategy_careless fst_strat :=
---   by
---   intro fst_strat f_act hist
---   cases' hist with head tail
---   · dsimp
---     rw [if_pos (by rfl)]
---     rw [if_neg (by exact List.cons_ne_nil f_act [])]
---     sorry
---   · dsimp
---     rw [if_neg (by exact List.cons_ne_nil head tail)]
---     rw [if_neg (by exact List.cons_ne_nil head (tail ++ [f_act]))]
-
-
---#exit
-
-
--- lemma bgrbgwrj
---   (g: Game_World α β)
---   (fst_act: β)
---   (fst_act_legal: g.fst_legal [] fst_act)
---   --(hmm : g.law_blind_fst)
---   (s_strat : Strategy α β)
---   (s_leg: ∀ f_start : Strategy α β , Strategy_legal (g.world_after_fst fst_act).init_game_state (fun x => (g.world_after_fst fst_act).snd_legal) f_strat s_strat s_strat)
---   -- maybe name this property ? = legal for all strategies ?
---   :
---   let fst_strat : Strategy α β := (fun ini hist => if hist = [] then fst_act else s_strat (g.world_after_fst fst_act).init_game_state (hist.dropLast)) ;
---   Strategy_legal g.init_game_state (fun x => g.fst_legal) fst_strat s_strat fst_strat :=
---   by
---   intro fst_strat t
---   induction' t with t ih
---   · dsimp [History_on_turn]
---     rw [if_pos (by rfl)]
---     exact fst_act_legal
---   · dsimp [fst_strat]
---     rw [if_neg _]
---     swap
---     · dsimp [History_on_turn]
---       split_ifs <;> decide
---     · rw [Game_World.world_after_fst_snd_legal] at s_leg
---       sorry
-
-
-lemma Game_World.History_of_preconditioned
-  (g: Game_World α β)
-  (fst_act: β)
-  (f_strat s_strat : Strategy α β)
-  (turn : ℕ):
-  let fst_strat : Strategy α β := (fun ini hist => if hist = [] then fst_act else s_strat (g.world_after_fst fst_act).init_game_state (hist.dropLast)) ;
-  let snd_strat : Strategy α β := (fun ini hist => f_strat (g.world_after_fst fst_act).init_game_state (hist.dropLast)) ;
-  History_on_turn g.init_game_state fst_strat snd_strat (turn + 1) =
-  (History_on_turn (g.world_after_fst fst_act).init_game_state f_strat s_strat turn) ++ [fst_act] :=
-  by
-  intro fst_strat snd_strat
-  induction' turn with t ih
-  · dsimp [History_on_turn, Turn_fst]
-    rw [if_pos (by decide), if_pos (by rfl)]
-  · dsimp only [History_on_turn] at *
-    by_cases q : Turn_fst (t+1)
-    · rw [Turn_fst_not_step] at q
-      rw [if_neg q] at *
-      rw [← Turn_fst_not_step] at q
-      rw [if_pos q, if_pos q] at *
-      rw [List.cons_append, ← ih]
-      congr
-      dsimp at ih
-      rw [← Game_World.world_after_fst_init] at ih
-      rw [ih]
-      rw [List.dropLast_concat]
-    · rw [if_neg q, if_neg q] at *
-      rw [Turn_fst_not_step, not_not] at q
-      rw [if_pos q] at *
-      rw [if_neg (by apply List.cons_ne_nil)]
-      rw [List.cons_append, ← ih]
-      congr
-      dsimp at ih
-      rw [← Game_World.world_after_fst_init] at ih
-      rw [ih]
-      rw [List.dropLast_concat]
-
-
-lemma Game_World.fst_of_preconditioned
-  (g: Game_World α β)
-  (fst_act: β)
-  (f_strat s_strat : Strategy α β)
-  (turn : ℕ):
-  let fst_strat : Strategy α β := (fun ini hist => if hist = [] then fst_act else s_strat (g.world_after_fst fst_act).init_game_state (hist.dropLast)) ;
-  let snd_strat : Strategy α β := (fun ini hist => f_strat (g.world_after_fst fst_act).init_game_state (hist.dropLast)) ;
-  fst_strat g.init_game_state (History_on_turn g.init_game_state fst_strat snd_strat (turn + 1)) =
-  s_strat (g.world_after_fst fst_act).init_game_state (History_on_turn (g.world_after_fst fst_act).init_game_state f_strat s_strat turn) :=
-  by
-  intro fst_strat snd_strat
-  dsimp [fst_strat]
-  rw [if_neg (by apply History_on_turn_nonempty_of_succ)]
-  have := g.History_of_preconditioned fst_act f_strat s_strat turn
-  dsimp at this
-  rw [this]
-  rw [List.dropLast_concat]
-
-
-
-lemma Game_World.snd_of_preconditioned
-  (g: Game_World α β)
-  (fst_act: β)
-  (f_strat s_strat : Strategy α β)
-  (turn : ℕ):
-  let fst_strat : Strategy α β := (fun ini hist => if hist = [] then fst_act else s_strat (g.world_after_fst fst_act).init_game_state (hist.dropLast)) ;
-  let snd_strat : Strategy α β := (fun ini hist => f_strat (g.world_after_fst fst_act).init_game_state (hist.dropLast)) ;
-  snd_strat g.init_game_state (History_on_turn g.init_game_state fst_strat snd_strat (turn + 1)) =
-  f_strat (g.world_after_fst fst_act).init_game_state (History_on_turn (g.world_after_fst fst_act).init_game_state f_strat s_strat turn) :=
-  by
-  intro fst_strat snd_strat
-  dsimp [fst_strat]
-  have := g.History_of_preconditioned fst_act f_strat s_strat turn
-  dsimp at this
-  rw [this]
-  rw [List.dropLast_concat]
-
-
-#check Game_World.world_after_fst_History
-
--- lemma Game_World.fst_preconditioned_careless
---   (g: Game_World α β)
---   (fst_act: β)
---   (f_strat s_strat : Strategy α β)
---   (hs : (g.world_after_fst fst_act).Strategy_careless s_strat) (hf : (g.world_after_fst fst_act).Strategy_careless f_strat)
---   (partiallity_hack : fst_act = s_strat (g.world_after_fst fst_act).init_game_state [])
---   -- shouldn't be a problem, as we may s_strat isn't used on empty history
---   (turn : ℕ):
---   let fst_strat : Strategy α β := (fun ini hist => if hist = [] then fst_act else s_strat (g.world_after_fst fst_act).init_game_state (hist.dropLast)) ;
---   g.Strategy_careless fst_strat :=
---   by
---   intro fst_strat act hist
---   dsimp
---   by_cases q : hist = []
---   · rw [if_pos q, if_neg (by apply List.append_ne_nil_of_ne_nil_right ; exact List.cons_ne_nil act [])]
---     rw [List.dropLast_concat, q]
---     exact partiallity_hack
---   · dsimp [Strategy_careless] at hs
---     rw [if_neg q, if_neg (by exact List.append_ne_nil_of_left_ne_nil hist [act] q), List.dropLast_concat]
---     rw [hs]
-    -- maybe just false ?
-
-
---#exit
-
-lemma Game_World.fst_legal_preconditioned
-  (g: Game_World α β)
-  (fst_act: β)
-  (fst_act_legal: g.fst_legal [] fst_act)
-  (f_strat s_strat : Strategy α β)
-  (hs : g.Strategy_careless s_strat) (hf : g.Strategy_careless f_strat)
-  (s_leg: Strategy_legal (g.world_after_fst fst_act).init_game_state (fun x => (g.world_after_fst fst_act).snd_legal) f_strat s_strat s_strat)
-  (partiallity_hack : s_strat g.init_game_state [] = fst_act)
-  -- should never be reqiested of s_strat, as its meant to be played on (g.world_after_fst fst_act)
-  -- TODO: show that one can assume this wlog on actual games
-  (b : g.law_blind_fst s_strat f_strat)
-  -- maybe can be derived from g.law_blind_fst fst_strat snd_strat ?
-  :
-  let fst_strat : Strategy α β := (fun ini hist => if hist = [] then fst_act else s_strat (g.world_after_fst fst_act).init_game_state (hist.dropLast)) ;
-  let snd_strat : Strategy α β := (fun ini hist => f_strat (g.world_after_fst fst_act).init_game_state (hist.dropLast)) ;
-  Strategy_legal g.init_game_state (fun x => g.fst_legal) fst_strat snd_strat fst_strat :=
-  by
-  intro fst_strat snd_strat t
-  induction' t with t ih
-  · dsimp [History_on_turn]
-    rw [if_pos (by rfl)]
-    exact fst_act_legal
-  · dsimp [fst_strat]
-    rw [if_neg _]
-    swap
-    · dsimp [History_on_turn]
-      split_ifs <;> decide
-    · have := g.History_of_preconditioned fst_act f_strat s_strat t
-      dsimp at this
-      rw [this]
-      rw [List.dropLast_concat]
-      rw [← Game_World.world_after_fst_init]
-      rw [← partiallity_hack]
-      rw [Game_World.world_after_fst_History]
-      · rw [← b]
-        rw [partiallity_hack]
-        apply s_leg
-      · exact hf
-      · exact hs
-
-
-lemma Game_World.snd_legal_preconditioned
-  (g: Game_World α β)
-  (fst_act: β)
-  (f_strat s_strat : Strategy α β)
-  (hs : g.Strategy_careless s_strat) (hf : g.Strategy_careless f_strat)
-  (f_leg: Strategy_legal (g.world_after_fst fst_act).init_game_state (fun x => (g.world_after_fst fst_act).fst_legal) f_strat s_strat f_strat)
-  (partiallity_hack : s_strat g.init_game_state [] = fst_act)
-  -- should never be reqiested of s_strat, as its meant to be played on (g.world_after_fst fst_act)
-  -- TODO: show that one can assume this wlog on actual games
-  (partiallity_hack' : snd_legal g [] (f_strat (world_after_fst g fst_act).init_game_state []))
-  -- again, should be assumed wlog, since this should be the first turn, so the snd law will never be asked to apply
-  (b : g.law_blind_snd s_strat f_strat)
-  -- maybe can be derived from g.law_blind_snd fst_strat snd_strat ?
-  :
-  let fst_strat : Strategy α β := (fun ini hist => if hist = [] then fst_act else s_strat (g.world_after_fst fst_act).init_game_state (hist.dropLast)) ;
-  let snd_strat : Strategy α β := (fun ini hist => f_strat (g.world_after_fst fst_act).init_game_state (hist.dropLast)) ;
-  Strategy_legal g.init_game_state (fun x => g.snd_legal) fst_strat snd_strat snd_strat :=
-  by
-  intro fst_strat snd_strat t
-  induction' t with t ih
-  · dsimp [History_on_turn]
-    rw [← Game_World.world_after_fst_init]
-    exact partiallity_hack'
-  · dsimp
-    have := g.History_of_preconditioned fst_act f_strat s_strat t
-    dsimp at this
-    rw [this]
-    rw [List.dropLast_concat]
-    rw [← Game_World.world_after_fst_init]
-    rw [← partiallity_hack]
-    rw [Game_World.world_after_fst_History]
-    · dsimp [law_blind_snd] at b
-      rw [← b]
-      rw [partiallity_hack]
-      apply f_leg
-    · exact hf
-    · exact hs
-
-
-
-def Game_World.must_terminate_before_wCarelessBlind {α β : Type u} (g : Game_World α β) (T : ℕ): Prop :=
-  ∀ f_strat s_strat : Strategy α β,
-  (f_law : Strategy_legal g.init_game_state (fun _ => g.fst_legal) f_strat s_strat f_strat) →
-  (s_law : Strategy_legal g.init_game_state (fun _ => g.snd_legal) f_strat s_strat s_strat) →
-  (hf : g.Strategy_careless f_strat) →
-  (hs : g.Strategy_careless s_strat) →
-  (hg : g.law_blind f_strat s_strat) →
-  let G := ({g with fst_strat := f_strat, fst_lawful := f_law, snd_strat := s_strat, snd_lawful := s_law} : Game α β) ;
-  ∃ turn ≤ T,
-    ((Turn_fst turn ∧ ∀ act : β, ¬ (G.fst_legal (G.history_on_turn turn) act))
-     ∨
-     (Turn_snd turn ∧ ∀ act : β, ¬ (G.snd_legal (G.history_on_turn turn) act)))
-
-
---#exit
-
-lemma Game_World.world_after_fst_init_must_terminate {α β : Type u} (g : Game_World α β)
-  (fst_act : β) (fst_act_legal : g.fst_legal [] fst_act)
-  {T : ℕ} :
-  g.must_terminate_before_wCarelessBlind (T + 1) → (g.world_after_fst fst_act).must_terminate_before_wCarelessBlind (T) :=
-  by
-  intro g_bnd
-  intro f_strat s_strat f_leg s_leg hf hs hg G
-  let fst_strat : Strategy α β := (fun ini hist => if hist = [] then fst_act else s_strat (g.world_after_fst fst_act).init_game_state (hist.dropLast))
-  let snd_strat : Strategy α β := (fun ini hist => f_strat (g.world_after_fst fst_act).init_game_state (hist.dropLast))
-  by_contra! con
-  specialize g_bnd fst_strat snd_strat
-  sorry
-
-
---#exit
-
--- lemma Game_World.world_after_fst_init_must_playable {α β : Type u} (g : Game_World α β)
---   (f_strat : Strategy α β) :
---   g.playable_snd → (g.world_after_fst (f_strat g.init_game_state [])).playable_fst :=
---   by
---   intro hp
---   obtain ⟨s, s_prop ⟩ := hp
---   use s
---   use f_strat
---   constructor
---   · apply Game_World.world_after_snd_legal
-
-
-  -- first strat would be second init strat with fst move the reaction to init fst strat
-
-
--- # New approach here
-
-def Strategy_legal_in_pair {α β : Type u}
-  (ini : α) (f_law s_law : α → List β → (β → Prop)) (f_strat s_strat : Strategy α β): Prop :=
-  ∀ turn : ℕ, (f_law ini (History_on_turn ini f_strat s_strat turn) (f_strat ini (History_on_turn ini f_strat s_strat turn)))
-    ∧ (s_law ini (History_on_turn ini f_strat s_strat turn) (s_strat ini (History_on_turn ini f_strat s_strat turn)))
-
-lemma Game_World.legal_copy {α β : Type u} (g : Game_World α β)
-  (fst_act : β) (fst_act_legal : g.fst_legal [] fst_act)
-  (f_strat s_strat : Strategy α β)
-  (f_leg: Strategy_legal (g.world_after_fst fst_act).init_game_state (fun x => (g.world_after_fst fst_act).fst_legal) f_strat s_strat f_strat)
-  (s_leg: Strategy_legal (g.world_after_fst fst_act).init_game_state (fun x => (g.world_after_fst fst_act).snd_legal) f_strat s_strat s_strat)
-  (hg : g.law_blind f_strat s_strat) :
-  let H := History_on_turn (g.world_after_fst fst_act).init_game_state f_strat s_strat
-  let fst_strat : Strategy α β := (fun ini hist => if hist = [] then fst_act else s_strat (g.world_after_fst fst_act).init_game_state (H (hist.length - 1)))
-  let snd_strat : Strategy α β := (fun ini hist => f_strat (g.world_after_fst fst_act).init_game_state (H (hist.length - 1)))
-  Strategy_legal_in_pair g.init_game_state (fun _ => g.fst_legal) (fun _ => g.snd_legal) fst_strat snd_strat :=
-  by
-  intro H fst_strat snd_strat t
-  induction' t with t ih
-  · dsimp [History_on_turn]
-    rw [if_pos (by rfl)]
-    exact fst_act_legal
-  · dsimp [fst_strat]
-    rw [if_neg (by apply History_on_turn_nonempty_of_succ)]
-
-
-
-lemma Game_World.world_after_fst_init_must_terminate' {α β : Type u} (g : Game_World α β)
-  (fst_act : β) (fst_act_legal : g.fst_legal [] fst_act)
-  {T : ℕ} :
-  g.must_terminate_before (T + 1) → (g.world_after_fst fst_act).must_terminate_before (T) :=
-  by
-  intro g_bnd
-  intro f_strat s_strat f_law s_law G
-  let H := History_on_turn (g.world_after_fst fst_act).init_game_state f_strat s_strat
-  let fst_strat : Strategy α β := (fun ini hist => if hist = [] then fst_act else s_strat (g.world_after_fst fst_act).init_game_state (H (hist.length - 1)))
-  let snd_strat : Strategy α β := (fun ini hist => f_strat (g.world_after_fst fst_act).init_game_state (H (hist.length - 1)))
-  by_contra! con
-  specialize g_bnd fst_strat snd_strat
-  sorry
-
-
-#exit
-
-lemma Game_World.conditioning {α β : Type u}
-  (g : Game_World α β)
-  --(hp : g.playable') (hpU : ∀ f_act, (g.world_after_fst f_act).playable') -- can we weaken this ?
-  -- probably not ? One can think of an f_act that causes the second player to have no legal moves
-  -- on the second round already. The game would still be playble, but the first player
-  -- has to avoid f_act.
-  {T : ℕ} (hg : g.must_terminate_before T)
-  {P : Game_World α β → Prop}
-  (step : ∀ (g' : Game_World α β), (∀ (f_strat : Strategy α β), P (g'.world_after_fst (f_strat g'.init_game_state []))) → P g')
-  (base : ∀ (g' : Game_World α β), g'.must_terminate_before 0 → P g')
-  :
-  P g :=
-  by
-  revert g
-  induction' T with T ih
-  · apply base
-  · intro g gt
-    apply step
-    intro f_strat
-    apply ih
-  -- · intro g hp hpU hg
-  --   obtain ⟨f, s, f_prop, s_prop ⟩ := hp
-  --   dsimp [Game_World.must_terminate_before] at hg
-  --   specialize hg f s (f_prop) (s_prop)
-  --   obtain ⟨z,zz, z_prop⟩ := hg
-  --   rw [Nat.le_zero] at zz
-  --   rw [zz] at z_prop
-  --   cases' z_prop with l r
-  --   · rw [Turn_fst] at l ; obtain ⟨ahh, b⟩ := l ; contradiction
-  --   · specialize s_prop
-  --     rw [Strategy_legal] at s_prop
-  --     specialize s_prop 0
-  --     exfalso
-  --     exact (r.2 (s g.init_game_state (History_on_turn g.init_game_state f s 0))) s_prop
-  -- · intro g hp hpU hg
-  --   apply ch
-  --   intro f_act
-  --   apply ih
-
-
-
-#exit
-
-theorem Game_World.Zermelo {α β : Type u} (g : Game_World α β)
-            (hp : g.playable)
-            {T : ℕ} (hg : g.must_terminate_before T) :
-            g.has_win_loose_draw_strat :=
-  by
-  revert g
-  induction' T with max_turn ih
-  · intro g hp hg
-    obtain ⟨⟨f, f_prop ⟩,⟨s, s_prop ⟩⟩ := hp
-    dsimp [Game_World.must_terminate_before] at hg
-    specialize hg f s (f_prop s) (s_prop f)
-    obtain ⟨z,zz, z_prop⟩ := hg
-    rw [Nat.le_zero] at zz
-    rw [zz] at z_prop
-    cases' z_prop with l r
-    · rw [Turn_fst] at l ; obtain ⟨ahh, b⟩ := l ; contradiction
-    · specialize s_prop f
-      rw [Strategy_legal] at s_prop
-      specialize s_prop 0
-      exfalso
-      exact (r.2 (s g.init_game_state (History_on_turn g.init_game_state f s 0))) s_prop
-  · intro g hp hg
-
--- do a by cases
-
--- show that g.world_after_fst are playable
--- show that g.world_after_fst must terminate bofre max_t
--- show that if g.world_after_fst is wld, the so is g
+    exact zGame_World.conditioning_bound g bd f_act f_leg
